@prefix : <https://w3id.org/pink/matter#> .
@prefix owl: <http://www.w3.org/2002/07/owl#> .
@prefix pav: <http://purl.org/pav/> .
@prefix rdf: <http://www.w3.org/1999/02/22-rdf-syntax-ns#> .
@prefix xml: <http://www.w3.org/XML/1998/namespace> .
@prefix xsd: <http://www.w3.org/2001/XMLSchema#> .
@prefix accr: <http://publications.europa.eu/resource/authority/access-right/> .
@prefix dcam: <http://purl.org/dc/dcam/> .
@prefix dcat: <http://www.w3.org/ns/dcat#> .
@prefix ddoc: <https://w3id.org/emmo/application/datadoc#> .
@prefix emmo: <https://w3id.org/emmo/hume#> .
@prefix foaf: <http://xmlns.com/foaf/0.1/> .
@prefix pink: <https://w3id.org/pink#> .
@prefix prov: <http://www.w3.org/ns/prov#> .
@prefix rdfs: <http://www.w3.org/2000/01/rdf-schema#> .
@prefix skos: <http://www.w3.org/2004/02/skos/core#> .
@prefix vann: <http://purl.org/vocab/vann/> .
@prefix dcatap: <http://data.europa.eu/r5r/> .
@prefix dcterms: <http://purl.org/dc/terms/> .
@prefix widoco: <https://w3id.org/widoco/vocab#> .
@base <https://w3id.org/pink/matter#> .

<https://w3id.org/pink/matter> rdf:type owl:Ontology ;
                                owl:versionIRI <https://w3id.org/pink/0.0.1/matter> ;
                                dcterms:abstract "The Matter module of PINK Annotation Schema providing a taxonomy for physical matter (including nanomaterial, chemical compounds, etc...) with anchor points for links for CheBI."@en ;
    dcterms:title "The Matter module of PINK Annotation Schema"@en ;
    widoco:introduction """
This module is a part of the [PINK Annotation Schema](https://pink-project.github.io/PINK-annotation-schema/widoco/index-en.html).
Matter is a physical entity that possess mass and occupies volume.

This module provides a categorisation of different types of matter entities.
At the top it categorise matter into molecular entities (discrete atoms or molecules) and different types of substances (homogenious properties).

A page illustrating showing how the PINK Annotation Schema categorise models can be found [here](https://pink-project.github.io/PINK-annotation-schema/docs/matter.html).
"""@en .


#################################################################
#    Annotation properties
#################################################################

###  http://purl.org/dc/terms/abstract
dcterms:abstract rdf:type owl:AnnotationProperty .


###  http://purl.org/dc/terms/title
dcterms:title rdf:type owl:AnnotationProperty .


###  http://www.w3.org/2004/02/skos/core#altLabel
skos:altLabel rdf:type owl:AnnotationProperty .


###  http://www.w3.org/2004/02/skos/core#definition
skos:definition rdf:type owl:AnnotationProperty .


###  http://www.w3.org/2004/02/skos/core#example
skos:example rdf:type owl:AnnotationProperty .


###  http://www.w3.org/2004/02/skos/core#prefLabel
skos:prefLabel rdf:type owl:AnnotationProperty .


###  http://www.w3.org/2004/02/skos/core#scopeNote
skos:scopeNote rdf:type owl:AnnotationProperty .


#################################################################
#    Classes
#################################################################

###  https://w3id.org/emmo/hume#AmorphousMaterial
emmo:AmorphousMaterial rdf:type owl:Class ;
                       rdfs:subClassOf emmo:MaterialByStructure ;
                       skos:altLabel "NonCrystallineMaterial"@en ;
                       skos:definition "A solid lacking a repeating, ordered atomic structure (long-range order)."@en ;
                       skos:prefLabel "AmorphousMaterial"@en ;
                       skos:scopeNote "A amorphous material resembles a frozen liquid with atoms arranged randomly, unlike crystalline solids with periodic patterns, leading to properties like no sharp melting point, irregular shapes, and isotropic characteristics (uniform properties in all directions)."@en .


###  https://w3id.org/emmo/hume#ArtificialMaterial
emmo:ArtificialMaterial rdf:type owl:Class ;
                        rdfs:subClassOf emmo:MaterialByOrigin ;
                        skos:definition "Any substance engineered or created by humans, often to mimic or improve upon natural materials."@en ;
                        skos:prefLabel "ArtificialMaterial"@en ;
                        skos:scopeNote "Artificial materials are typically engineered through chemical synthesis from natural raw materials like oil or coal, resulting in polymers such as plastics, nylon, or polyester, designed for specific, enhanced properties like strength, durability, or moldability not found in nature."@en .


###  https://w3id.org/emmo/hume#Atom
emmo:Atom rdf:type owl:Class ;
    rdfs:subClassOf emmo:MolecularEntity ;
    skos:altLabel "ChemicalElement"@en ;
    skos:prefLabel "Atom"@en ;
    skos:definition """A standalone atom has direct part one 'nucleus' and one 'electron_cloud'.

An O 'atom' within an O₂ 'molecule' is an 'e-bonded_atom'.

In this material branch, H atom is a particular case, with respect to higher atomic number atoms, since as soon as it shares its electron it has no nucleus entangled electron cloud.

We cannot say that H₂ molecule has direct part two H atoms, but has direct part two H nucleus."""@en ;
    skos:scopeNote "An 'atom' is a 'nucleus' surrounded by an 'electron_cloud', i.e. a quantum system made of one or more bounded electrons."@en .


###  https://w3id.org/emmo/hume#BondedAtom
emmo:BondedAtom rdf:type owl:Class ;
                rdfs:subClassOf emmo:Atom ;
                skos:definition "A bonded atom that shares at least one electron to the atom-based entity of which is part of."@en ;
                skos:prefLabel "BondedAtom"@en ;
                skos:scopeNote """A real bond between atoms is always something hybrid between covalent, metallic and ionic.

In general, metallic and ionic bonds have atoms sharing electrons."""@en ,
                               "The bond types that are covered by this definition are the strong electronic bonds: covalent, metallic and ionic."@en ,
                               "This class can be used to represent molecules as simplified quantum systems, in which outer molecule shared electrons are un-entangled with the inner shells of the atoms composing the molecule."@en .


###  https://w3id.org/emmo/hume#CeramicMaterial
emmo:CeramicMaterial rdf:type owl:Class ;
                     rdfs:subClassOf emmo:MaterialByType ;
                     skos:altLabel "Ceramic"@en ;
                     skos:definition "An inorganic non-metallic solid made from elements (metals, non-metals, semi-metals like silicon) combined into compounds (oxides, carbides, nitrides) that are typically hard, strong, brittle, corrosion-resistant, and good insulators."@en ;
                     skos:prefLabel "CeramicMaterial"@en ;
                     skos:scopeNote "Ceramic materials are hardened by intense heat and typically used from pottery and tiles to advanced electronics and aerospace parts."@en .



###  https://w3id.org/emmo/hume#ChemicalCompound
emmo:ChemicalCompound rdf:type owl:Class ;
    rdfs:subClassOf emmo:ChemicalSubstance ;
    skos:prefLabel "ChemicalCompound"@en ;
    skos:definition "A chemical substance composed of many identical molecules (or molecular entities) composed of atoms from more than one element held together by chemical bonds."@en ;
    rdfs:seeAlso "https://en.wikipedia.org/wiki/Chemical_compound"@en .

###  https://w3id.org/emmo/hume#InorganicCompound
emmo:InorganicCompound rdf:type owl:Class ;
    rdfs:subClassOf emmo:ChemicalCompound ;
    skos:prefLabel "InorganicCompound"@en ;
    skos:definition "A chemical compound that is not organic."@en ;
    rdfs:seeAlso "https://en.wikipedia.org/wiki/Inorganic_compound"@en .

###  https://w3id.org/emmo/hume#OrganicCompound
emmo:OrganicCompound rdf:type owl:Class ;
    rdfs:subClassOf emmo:ChemicalCompound ;
    skos:prefLabel "OrganicCompound"@en ;
    skos:definition "A chemical compound containing carbon atoms."@en ;
    skos:scopeNote "The definition of organic compound is based on the IUPAC Gold Book. However, sometimes an organic compound is defined as a chemical compound that contains a carbon-hydrogen or carbon-carbon bond. Also, some carbon-containing compounds are typically not classified as organic, like carbides, carbonates, and cyanides."@en ;
    rdfs:seeAlso "https://en.wikipedia.org/wiki/Organic_compound"@en .


###  https://w3id.org/emmo/hume#ChemicalEntity
emmo:ChemicalEntity rdf:type owl:Class ;
    skos:scopeNote """A chemical entity comprises the two different ways to represents matter: as single recognizable particle entity (molecular entity) and as a composition of particle entities (substance).

This distinction is not well assessed in actual chemical nomenclature, in which an element name refers to both the pure elemental substance or the atom.

In the EMMO we force the adoption of a more strict categorization based on mereotopology.

The class Material hosts the subclasses for which a substance can be identified without necessarily considering its nature of molecule/atom or substance (e.g. hydrocarbon is the class of both hydrocarbon molecules or gases)."""@en ;
    skos:definition "The union of ChemicalSubstance and MolecularEntity."@en ;
    skos:prefLabel "ChemicalEntity"@en .

###  https://w3id.org/emmo/hume#ChemicalSubstance
emmo:ChemicalSubstance rdf:type owl:Class ;
                       rdfs:subClassOf emmo:ChemicalEntity ,
                                       emmo:Substance ;
    owl:disjointWith emmo:MolecularEntity ;
    skos:scopeNote "A chemical substance is always composed of more than one molecular entity. It lays in the continuum or mesoscopic domain."@en ;
    rdfs:subClassOf emmo:Substance ;
    skos:prefLabel "ChemicalSubstance"@en ;
    skos:definition "Matter of constant composition best characterized by the entities (molecules, formula units, atoms) it is composed of."@en ;
    rdfs:seeAlso "https://doi.org/10.1351/goldbook.C01039"@en .


###  https://w3id.org/emmo/hume#CompactMaterial
emmo:CompactMaterial rdf:type owl:Class ;
                     rdfs:subClassOf emmo:MaterialByCompactness, emmo:Solid ;
                     skos:prefLabel "CompactMaterial"@en ;
    skos:definition "A solid material whose particles are closely and firmly packed together, resulting in a high density, solid structure without significant internal voids or cavities."@en .

###  https://w3id.org/emmo/hume#CompositeMaterial
emmo:CompositeMaterial rdf:type owl:Class ;
                       rdfs:subClassOf emmo:MaterialByType ;
                       skos:altLabel "Composite"@en ;
                       skos:definition "A material that contains two or more constituent materials."@en ;
                       skos:prefLabel "CompositeMaterial"@en .


###  https://w3id.org/emmo/hume#CondensedMatter
emmo:CondensedMatter rdf:type owl:Class ;
    rdfs:subClassOf emmo:StateOfMatter ;
    skos:prefLabel "CondensedMatter"@en ;
    skos:definition "Solid or liquid matter."@en ;
    skos:scopeNote "The subject of condensed matter physics that deals with the macroscopic and microscopic physical properties of matter, especially the solid and liquid phases which arise from electromagnetic forces between atoms. More generally, the subject deals with \"condensed\" phases of matter: systems of many constituents with strong interactions between them."@en .


###  https://w3id.org/emmo/hume#ContinuumSubstance
emmo:ContinuumSubstance rdf:type owl:Class ;
                        rdfs:subClassOf emmo:Substance ;
    owl:disjointWith emmo:MesoscopicSubstance ;
    skos:prefLabel "ContinuumSubstance"@en ;
    skos:definition """A state that is a collection of sufficiently large number of other parts such that:
- it is the bearer of qualities that can exists only by the fact that it is a sum of parts
- the smallest partition dV of the state volume in which we are interested in, contains enough parts to be statistically consistent: n [#/m3] x dV [m3] >> 1"""@en ;
    skos:scopeNote "A continuum is made of a sufficient number of parts that it continues to exists as continuum individual even after the loss of one of them i.e. a continuum is a redundant."@en,
        """A continuum is not necessarily small (i.e. composed by the minimum amount of sates to fulfill the definition).

A single continuum individual can be the whole fluid in a pipe."""@en,
        "A continuum is the bearer of properties that are generated by the interactions of parts such as viscosity and thermal or electrical conductivity."@en .


###  https://w3id.org/emmo/hume#CrystallineMaterial
emmo:CrystallineMaterial rdf:type owl:Class ;
                         rdfs:subClassOf emmo:MaterialByStructure , emmo:Solid ;
    skos:prefLabel "CrystallineMaterial"@en ;
    skos:definition "A solid where atoms, ions, or molecules are arranged in a highly ordered, repeating, three-dimensional pattern, forming a crystal lattice that extends throughout the substance, giving it characteristic geometric shapes and distinct physical properties like sharp melting points, unlike amorphous solids with random structures."@en .


###  https://w3id.org/emmo/hume#ElementalSubstance
emmo:ElementalSubstance rdf:type owl:Class ;
                        rdfs:subClassOf emmo:ChemicalSubstance ;
    skos:altLabel "PureSubstance"@en ;
    skos:prefLabel "ElementalSubstance"@en ;
    skos:definition "A chemical substance composed of atoms with the same number of protons in the atomic nucleus."@en ;
    rdfs:seeAlso "https://doi.org/10.1351/goldbook.C01022"@en .


###  https://w3id.org/emmo/hume#Fluid
emmo:Fluid rdf:type owl:Class ;
    rdfs:subClassOf emmo:StateOfMatter ;
    skos:example "Gas, liquid, plasma,"@en ;
    skos:prefLabel "Fluid"@en ;
    skos:definition "A continuum that has no fixed shape and yields easily to external pressure."@en .


###  https://w3id.org/emmo/hume#Gas
emmo:Gas rdf:type owl:Class ;
    rdfs:subClassOf emmo:Fluid ;
    skos:prefLabel "Gas"@en ;
    skos:definition "Gas is a compressible fluid, a state of matter that has no fixed shape and no fixed volume."@en .


###  https://w3id.org/emmo/hume#GranularMaterial
emmo:GranularMaterial rdf:type owl:Class ;
    rdfs:subClassOf emmo:MaterialByCompactness ;
    skos:prefLabel "GranularMaterial"@en ;
    skos:definition "A granular material is a conglomeration of discrete solid, macroscopic particles that are  large enough to avoid thermal motion fluctuations, and characterized by a loss of energy whenever the particles interact."@en .


###  https://w3id.org/emmo/hume#IonAtom
emmo:IonAtom rdf:type owl:Class ;
    rdfs:subClassOf emmo:StandaloneAtom ;
    skos:prefLabel "IonAtom"@en ;
    skos:definition "A standalone atom with an unbalanced number of electrons with respect to its atomic number."@en .


###  https://w3id.org/emmo/hume#Liquid
emmo:Liquid rdf:type owl:Class ;
            rdfs:subClassOf emmo:CondensedMatter ,
    emmo:Fluid ;
    skos:prefLabel "Liquid"@en ;
    skos:definition "A liquid is a nearly incompressible fluid that conforms to the shape of its container but retains a (nearly) constant volume independent of pressure."@en .


###  https://w3id.org/emmo/hume#ManufacturedMaterial
emmo:ManufacturedMaterial rdf:type owl:Class ;
                          rdfs:subClassOf emmo:ArtificialMaterial .


###  https://w3id.org/emmo/hume#Material
emmo:Material rdf:type owl:Class ;
    rdfs:subClassOf emmo:Substance ;
    skos:prefLabel "Material"@en ;
    skos:definition "The class of individuals standing for an amount of ordinary matter substance."@en ;
    skos:scopeNote "A instance of a material (e.g. nitrogen) can represent any state of matter. The fact that the individual also belongs to other classes (e.g. Gas) would reveal the actual form in which the material is found."@en,
        "A material may be either a mesoscopic or a continuum substance."@en,
        "Material usually means some definite kind, quality, or quantity of matter, especially as intended for use."@en .


###  https://w3id.org/emmo/hume#MaterialByClassicalMaterialsScience
emmo:MaterialByClassicalMaterialsScience rdf:type owl:Class ;
                                         rdfs:subClassOf emmo:Material .


###  https://w3id.org/emmo/hume#MaterialByCompactness
emmo:MaterialByCompactness rdf:type owl:Class ;
    rdfs:subClassOf emmo:Material ;
    skos:prefLabel "MaterialByCompactness"@en .


###  https://w3id.org/emmo/hume#MaterialByForceResponse
emmo:MaterialByForceResponse rdf:type owl:Class ;
                             rdfs:subClassOf emmo:Material .


###  https://w3id.org/emmo/hume#MaterialByFunction
emmo:MaterialByFunction rdf:type owl:Class ;
                        rdfs:subClassOf emmo:Material .


###  https://w3id.org/emmo/hume#MaterialByOrigin
emmo:MaterialByOrigin rdf:type owl:Class ;
    rdfs:subClassOf emmo:Material ;
    skos:prefLabel "MaterialByOrigin"@en .


###  https://w3id.org/emmo/hume#MaterialBySize
emmo:MaterialBySize rdf:type owl:Class ;
    rdfs:subClassOf emmo:Material ;
    skos:prefLabel "MaterialBySize"@en .


###  https://w3id.org/emmo/hume#MaterialByStructure
emmo:MaterialByStructure rdf:type owl:Class ;
    rdfs:subClassOf emmo:MaterialByClassicalMaterialsScience ;
    skos:prefLabel "MaterialByStructure"@en .


###  https://w3id.org/emmo/hume#MaterialByType
emmo:MaterialByType rdf:type owl:Class ;
                    rdfs:subClassOf emmo:MaterialByClassicalMaterialsScience ;
                    skos:definition "Categorisation of matter by its type."@en .


###  https://w3id.org/emmo/hume#MesoscopicSubstance
emmo:MesoscopicSubstance rdf:type owl:Class ;
                         rdfs:subClassOf emmo:Substance ;
                         skos:definition "A matter that is not a particulate matter and that does not fullfill the criteria of being a continuum substance."@en ;
                         skos:example """nanoparticle,
quantum dot,
carbon nanotupe"""@en ;
                         skos:prefLabel "MesoscopicSubstance"@en ;
                         skos:scopeNote "Mesoscopic substances typically exist on a length scale between atoms and molecules and macroscopic (bulk) substances. They are typically in the range of some nanometers to about a micrometer and often exhibit unique physical properties due to their size and shape."@en .


###  https://w3id.org/emmo/hume#MetallicMaterial
emmo:MetallicMaterial rdf:type owl:Class ;
                      rdfs:subClassOf emmo:MaterialByType ;
    skos:scopeNote
    "Metallic materials are known for their shiny luster, excellent electrical/thermal conductivity, malleability (shapable by hammering), and ductility (can be drawn into wires), due to metallic bonding (shared electrons); they often form alloys (like steel from iron/carbon) to enhance these properties for diverse applications."@en ;
    skos:prefLabel "MetallicMaterial"@en ;
    skos:definition "Inorganic substance, consisting of one or more metallic elements."@en .


###  https://w3id.org/emmo/hume#Mixture
emmo:Mixture rdf:type owl:Class ;
    rdfs:subClassOf emmo:ContinuumSubstance ;
    skos:prefLabel "Mixture"@en ;
    skos:definition "A continuum substance made up of two or more different substances which are physically (not chemically) combined."@en .


###  https://w3id.org/emmo/hume#MolecularEntity
emmo:MolecularEntity rdf:type owl:Class ;
    rdfs:subClassOf emmo:ChemicalEntity ;
    skos:prefLabel "MolecularEntity"@en ;
    skos:scopeNote """Molecular entity is used as a general term for singular entities, irrespective of their nature, while chemical species stands for sets or ensembles of molecular entities.

Note that the name of a compound may refer to the respective molecular entity or to the chemical species,"""@en ;
    skos:example "Hydrogen molecule is an adequate definition of a certain molecular entity for some purposes, whereas for others it is necessary to distinguish the electronic state and/or vibrational state and/or nuclear spin, etc. of the hydrogen molecule."@en ,
    "Methane, may mean a single molecule of CH4 (molecular entity) or a molar amount, specified or not (chemical species), participating in a reaction. The degree of precision necessary to describe a molecular entity depends on the context."@en ;
    skos:definition "Any constitutionally or isotopically distinct atom, molecule, ion, ion pair, radical, radical ion, complex, conformer etc., identifiable as a separately distinguishable entity that can undergo a chemical reaction."@en ;
    rdfs:isDefinedBy "https://goldbook.iupac.org/terms/view/M03986"@en .


###  https://w3id.org/emmo/hume#Molecule
emmo:Molecule rdf:type owl:Class ;
              rdfs:subClassOf emmo:MolecularEntity ;
    skos:example "H₂0, C₆H₁₂O₆, CH₄"@en ;
    skos:prefLabel "Molecule"@en ;
    skos:definition "An atom-based state defined by an exact number of e-bonded atomic species and an electron cloud made of the shared electrons."@en ;
    skos:scopeNote """An entity is called essential if removing one direct part will lead to a change in entity class.
An entity is called redundant if removing one direct part will not lead to a change in entity class."""@en,
        """This definition states that this object is a non-periodic set of atoms or a set with a finite periodicity.
Removing an atom from the state will result in another type of atom_based state.
e.g. you cannot remove H from H₂0 without changing the molecule type (essential). However, you can remove a C from a nanotube (redundant). C60 fullerene is a molecule, since it has a finite periodicity and is made of a well defined number of atoms (essential). A C nanotube is not a molecule, since it has an infinite periodicity (redundant)."""@en .


###  https://w3id.org/emmo/hume#NanoMaterial
emmo:NanoMaterial rdf:type owl:Class ;
                  rdfs:subClassOf emmo:MaterialBySize ;
    skos:prefLabel "NanoMaterial"@en ;
    skos:definition "Materials possessing at minimum one external dimension, or internal structure, in the range of 1-100nm."@en .

###  https://w3id.org/emmo/hume#NaturalMaterial
emmo:NaturalMaterial rdf:type owl:Class ;
    rdfs:subClassOf emmo:MaterialByOrigin ;
    skos:prefLabel "NaturalMaterial"@en ;
    skos:definition "A Material occurring in nature, without the need of human intervention."@en .


###  https://w3id.org/emmo/hume#NeutralAtom
emmo:NeutralAtom rdf:type owl:Class ;
                 rdfs:subClassOf emmo:StandaloneAtom ;
    owl:disjointWith emmo:IonAtom ;
    skos:prefLabel "NeutralAtom"@en ;
    skos:definition "A standalone atom that has no net charge."@en .


###  https://w3id.org/emmo/hume#PhaseOfMatter
emmo:PhaseOfMatter rdf:type owl:Class ;
    rdfs:subClassOf emmo:ContinuumSubstance ;
    skos:altLabel "Phase"@en ;
    skos:prefLabel "PhaseOfMatter"@en ;
    skos:definition "A matter object throughout which all physical properties of a material are essentially uniform."@en ;
    skos:scopeNote """In the physical sciences, a phase is a region of space (a thermodynamic system), throughout which all physical properties of a material are essentially uniform. Examples of physical properties include density, index of refraction, magnetization and chemical composition. A simple description is that a phase is a region of material that is chemically uniform, physically distinct, and (often) mechanically separable. In a system consisting of ice and water in a glass jar, the ice cubes are one phase, the water is a second phase, and the humid air is a third phase over the ice and water. The glass of the jar is another separate phase.

The term phase is sometimes used as a synonym for state of matter, but there can be several immiscible phases of the same state of matter. Also, the term phase is sometimes used to refer to a set of equilibrium states demarcated in terms of state variables such as pressure and temperature by a phase boundary on a phase diagram. Because phase boundaries relate to changes in the organization of matter, such as a change from liquid to solid or a more subtle change from one crystal structure to another, this latter usage is similar to the use of "phase" as a synonym for state of matter. However, the state of matter and phase diagram usages are not commensurate with the formal definition given above and the intended meaning must be determined in part from the context in which the term is used."""@en .


###  https://w3id.org/emmo/hume#Plasma
emmo:Plasma rdf:type owl:Class ;
    rdfs:subClassOf emmo:Fluid ;
    skos:prefLabel "Plasma"@en ;
    skos:definition "A fluid in which a gas is ionized to a level where its electrical conductivity allows long-range electric and magnetic fields to dominate its behaviour."@en .


###  https://w3id.org/emmo/hume#PolymericEntity
emmo:PolyAtomicEntity rdf:type owl:Class ;
    rdfs:subClassOf emmo:MolecularEntity ;
    skos:definition "An entity made of two or more bonded atoms."@en .


###  https://w3id.org/emmo/hume#PolymericMaterial
emmo:PolymericMaterial rdf:type owl:Class ;
    rdfs:subClassOf emmo:MaterialByType ;
    skos:prefLabel "PolymericMaterial"@en ;
    skos:definition "A substance made of macromolecules formed by linking many smaller, repeating chemical units called monomers into long chains or networks, resulting in unique properties like toughness, elasticity, or flexibility, found in both natural forms (like DNA, protein) and synthetic plastics, rubbers, and fibers."@en .



###  https://w3id.org/emmo/hume#Powder
emmo:Powder rdf:type owl:Class ;
    rdfs:subClassOf emmo:GranularMaterial ;
    rdfs:isDefinedBy "Duran, J., Reisinger A., Sands, Powders, and Grains: An Introduction to the Physics of Granular Materials. November 1999, Springer-Verlag New York, Inc., New York, ISBN 0-387-98656-1."@en ;
    skos:prefLabel "Powder"@en ;
    skos:definition "A powder is a granular material composed of many very fine dry solid particles that may flow freely when shaken or tilted."@en .


###  https://w3id.org/emmo/hume#Solid
emmo:Solid rdf:type owl:Class ;
    rdfs:subClassOf emmo:CondensedMatter ;
    skos:prefLabel "Solid"@en ;
    skos:definition "A continuum characterized by structural rigidity and resistance to changes of shape or volume, that retains its shape and density when not confined."@en .



###  https://w3id.org/emmo/hume#StandaloneAtom
emmo:StandaloneAtom rdf:type owl:Class ;
    rdfs:subClassOf emmo:Atom ;
    skos:prefLabel "StandaloneAtom"@en ;
    skos:definition "An atom that does not share electrons with other atoms."@en .


###  https://w3id.org/emmo/hume#StateOfMatter
emmo:StateOfMatter rdf:type owl:Class ;
    rdfs:subClassOf emmo:ContinuumSubstance ;
    skos:prefLabel "StateOfMatter"@en ;
    skos:definition "A superclass made as the disjoint union of all the form under which matter can exist."@en ;
    skos:scopeNote "In physics, a state of matter is one of the distinct forms in which matter can exist. Four states of matter are observable in everyday life: solid, liquid, gas, and plasma."@en ;
    owl:seeAlso <https://en.wikipedia.org/wiki/State_of_matter> .


###  https://w3id.org/emmo/hume#Substance
emmo:Substance rdf:type owl:Class ;
    skos:example "A litre of water."@en,
        "A pen can be classified as a substance (although it has parts with different properties) since it can be identified as being solid."@en ;
    skos:prefLabel "Substance"@en ;
    skos:definition "A matter entity characterised by the fact that it possesses some homogeneous properties or identification criteria."@en .


###  https://w3id.org/pink#AdvancedMaterial
pink:AdvancedMaterial rdf:type owl:Class ;
    rdfs:subClassOf emmo:ArtificialMaterial , emmo:MaterialByFunction ;
    skos:prefLabel "AdvancedMaterial"@en ;
    skos:definition "A designed material tailored to simultaneously meet two or more pre-defined criteria."@en .

###  https://w3id.org/pink#MacroMolecule
pink:MacroMolecule rdf:type owl:Class ;
    rdfs:subClassOf emmo:Molecule ;
    skos:prefLabel "MacroMolecule"@en ;
    skos:definition "A molecule with a specific weight larger than 5000 dalton."@en ;
    owl:seeAlso <https://en.wikipedia.org/wiki/Macromolecule> .

###  https://w3id.org/pink#MicroMolecule
pink:MicroMolecule rdf:type owl:Class ;
    rdfs:subClassOf emmo:Molecule ;
    skos:prefLabel "MicroMolecule"@en ;
    skos:definition "A molecule with a specific weight smaller than 1000 dalton."@en ;
    owl:seeAlso <https://en.wikipedia.org/wiki/Small_molecule> .

###  https://w3id.org/pink#Protein
pink:Protein rdf:type owl:Class ;
    rdfs:subClassOf emmo:Molecule ;
    skos:prefLabel "Protein"@en ;
    skos:definition "A large molecule made of long chains of amino acids."@en ;
    owl:seeAlso <https://en.wikipedia.org/wiki/Protein> .

###  https://w3id.org/pink#StructuralMaterial
pink:StructuralMaterial rdf:type owl:Class ;
    rdfs:subClassOf emmo:MaterialByFunction ;
    skos:prefLabel "StructuralMaterial"@en ;
    skos:definition "A material Designed to bear loads and provide mechanical strength, stiffness, and durability (e.g., steel for bridges, concrete for buildings, aerospace alloys)."@en .

###  https://w3id.org/pink#ElectronicMaterial
pink:ElectronicMaterial rdf:type owl:Class ;
    rdfs:subClassOf emmo:MaterialByFunction ;
    skos:prefLabel "ElectronicMaterial"@en ;
    skos:definition "A material for electronic applications, like silicon used in computer chips, solar cells, and circuits."@en .

###  https://w3id.org/pink#MagneticMaterial
pink:MagneticMaterial rdf:type owl:Class ;
    rdfs:subClassOf emmo:MaterialByFunction ;
    skos:prefLabel "MagneticMaterial"@en ;
    skos:definition "A material for magnetic applications, like for data storage, motors, and transformers (e.g., iron, ferrite)."@en .

###  https://w3id.org/pink#OpticalMaterial
pink:OpticalMaterial rdf:type owl:Class ;
    rdfs:subClassOf emmo:MaterialByFunction ;
    skos:prefLabel "OpticalMaterial"@en ;
    skos:definition "A material for optical applications. Designed for specific interactions with light, such as fiber optics, lasers, or transparent coatings."@en .

###  https://w3id.org/pink#EnergyMaterial
pink:EnergyMaterial rdf:type owl:Class ;
    rdfs:subClassOf emmo:MaterialByFunction ;
    skos:prefLabel "EnergyMaterial"@en ;
    skos:definition "A material for energy applications, including energy generation, storage, and conversion, such as batteries, supercapacitors, and fuel cells."@en .

###  https://w3id.org/pink#BiocompatibleMaterial
pink:BiocompatibleMaterial rdf:type owl:Class ;
    rdfs:subClassOf emmo:MaterialByFunction ;
    skos:prefLabel "BiocompatibleMaterial"@en ;
    skos:definition "Material designed to be biocompatible for implantation in the body, such as artificial joints or tissue scaffolds."@en .


###  https://w3id.org/pink#NanoParticle
pink:NanoParticle rdf:type owl:Class ;
    rdfs:subClassOf emmo:NanoMaterial ;
    skos:prefLabel "NanoParticle"@en ;
    skos:definition "A material with all dimensions in the range of 1-100 nm."@en ;
    skos:scopeNote "Nanoparticles are often considered to be 0-dimensional nanomaterials."@en ;
    owl:seeAlso <https://doi.org/10.3390/membranes10100297>, <https://en.wikipedia.org/wiki/Nanoparticle> .

###  https://w3id.org/pink#NanoFiber
pink:NanoFiber rdf:type owl:Class ;
    rdfs:subClassOf emmo:NanoMaterial ;
    skos:prefLabel "NanoFiber"@en ;
    skos:definition "A material with two dimensions in the range of 1-100 nm."@en ;
    skos:scopeNote "Nanofibers are often considered to be 1-dimensional nanomaterials."@en ;
    owl:seeAlso <https://doi.org/10.3390/membranes10100297>, <https://en.wikipedia.org/wiki/Nanofiber> .

###  https://w3id.org/pink#NanoPlate
pink:NanoPlate rdf:type owl:Class ;
    rdfs:subClassOf emmo:NanoMaterial ;
    skos:prefLabel "NanoPlate"@en ;
    skos:definition "A material with one dimension in the range of 1-100 nm."@en ;
    skos:scopeNote "Nanoplates are often considered to be 2-dimensional nanomaterials."@en ;
    owl:seeAlso <https://doi.org/10.3390/membranes10100297> .

###  https://w3id.org/pink#NanoStructuredMaterial
pink:NanoStructuredMaterial rdf:type owl:Class ;
    rdfs:subClassOf emmo:NanoMaterial ;
    skos:prefLabel "NanoStructuredMaterial"@en ;
    skos:definition "A material with at least one physically or chemically distinct region with at least one dimension in the range of 1-100 nm."@en ;
    skos:scopeNote "Nanostructured materials are considered to be 3-dimensional nanomaterials."@en ;
    owl:seeAlso <https://doi.org/10.3390/membranes10100297> .

###  https://w3id.org/pink#NanoTube
pink:NanoTube rdf:type owl:Class ;
    rdfs:subClassOf pink:NanoFiber ;
    skos:prefLabel "NanoTube"@en ;
    skos:definition "A hollow nanofiber."@en ;
    owl:seeAlso <https://en.wikipedia.org/wiki/Nanotube> .

###  https://w3id.org/pink#NanoRod
pink:NanoRod rdf:type owl:Class ;
    rdfs:subClassOf pink:NanoFiber ;
    skos:prefLabel "NanoRod"@en ;
    skos:definition "A solid nanofiber."@en ;
    owl:seeAlso <https://en.wikipedia.org/wiki/Nanorod> .

###  https://w3id.org/pink#NanoComposite
pink:NanoComposite rdf:type owl:Class ;
    rdfs:subClassOf pink:NanoStructuredMaterial , emmo:CompositeMaterial ;
    skos:prefLabel "NanoComposite"@en ;
    skos:definition "A composite material with at least one physically or chemically distinct region or collection of regions having at least one dimension in the range of 1-100 nm."@en ;
    owl:seeAlso <https://en.wikipedia.org/wiki/Nanocomposite> .



[] a owl:Axiom ;
    owl:annotatedProperty skos:scopeNote ;
    owl:annotatedSource emmo:PhaseOfMatter ;
    owl:annotatedTarget """In the physical sciences, a phase is a region of space (a thermodynamic system), throughout which all physical properties of a material are essentially uniform. Examples of physical properties include density, index of refraction, magnetization and chemical composition. A simple description is that a phase is a region of material that is chemically uniform, physically distinct, and (often) mechanically separable. In a system consisting of ice and water in a glass jar, the ice cubes are one phase, the water is a second phase, and the humid air is a third phase over the ice and water. The glass of the jar is another separate phase.

The term phase is sometimes used as a synonym for state of matter, but there can be several immiscible phases of the same state of matter. Also, the term phase is sometimes used to refer to a set of equilibrium states demarcated in terms of state variables such as pressure and temperature by a phase boundary on a phase diagram. Because phase boundaries relate to changes in the organization of matter, such as a change from liquid to solid or a more subtle change from one crystal structure to another, this latter usage is similar to the use of "phase" as a synonym for state of matter. However, the state of matter and phase diagram usages are not commensurate with the formal definition given above and the intended meaning must be determined in part from the context in which the term is used."""@en ;
    rdfs:seeAlso "https://en.wikipedia.org/wiki/Phase_(matter)"@en .

[] a owl:Axiom ;
    owl:annotatedProperty skos:scopeNote ;
    owl:annotatedSource emmo:CondensedMatter ;
    owl:annotatedTarget "The subject of condensed matter physics that deals with the macroscopic and microscopic physical properties of matter, especially the solid and liquid phases which arise from electromagnetic forces between atoms. More generally, the subject deals with \"condensed\" phases of matter: systems of many constituents with strong interactions between them."@en ;
    rdfs:seeAlso "https://en.wikipedia.org/wiki/Condensed_matter_physics"@en .




###  Generated by the OWL API (version 4.5.29.2024-05-13T12:11:03Z) https://github.com/owlcs/owlapi
