@prefix : <https://w3id.org/pink#> .
@prefix owl: <http://www.w3.org/2002/07/owl#> .
@prefix rdf: <http://www.w3.org/1999/02/22-rdf-syntax-ns#> .
@prefix xml: <http://www.w3.org/XML/1998/namespace> .
@prefix xsd: <http://www.w3.org/2001/XMLSchema#> .
@prefix bibo: <http://purl.org/ontology/bibo/> .
@prefix foaf: <http://xmlns.com/foaf/0.1/> .
@prefix rdfs: <http://www.w3.org/2000/01/rdf-schema#> .
@prefix dcat: <http://www.w3.org/ns/dcat#> .
@prefix skos: <http://www.w3.org/2004/02/skos/core#> .
@prefix prov: <http://www.w3.org/ns/prov#> .
@prefix vann: <http://purl.org/vocab/vann/> .
@prefix dcatap: <http://data.europa.eu/r5r/> .
@prefix dcterms: <http://purl.org/dc/terms/> .
@prefix dcat: <http://www.w3.org/ns/dcat#> .
@prefix widoco: <https://w3id.org/widoco/vocab#> .
@prefix ddoc: <https://w3id.org/emmo/application/datadoc#> .
@prefix emmo: <https://w3id.org/emmo/hume#> .
@prefix pink: <https://w3id.org/pink#> .

@base <https://w3id.org/pink#> .

<https://w3id.org/pink>
    rdf:type owl:Ontology ;
    owl:versionIRI <https://w3id.org/pink/0.0.1> ;
    owl:imports
        <https://w3id.org/pink/0.0.1/reused-terms> ,
        <https://w3id.org/pink/0.0.1/matter> ,
        <https://w3id.org/pink/0.0.1/models> ,
        <https://w3id.org/pink/0.0.1/cheminf-mappings> ,
        <https://w3id.org/pink/0.0.1/ssbd-taxonomy> ;
    dcatap:status "Under Development" ;
    dcterms:abstract """The PINK Annotation Schema provides the semantic basis for SSbD.

The PINK Annotation Schema expands on the annotation schema provided by tripper, which again expands on the DCAT-AP.

A reference documentation of terms reused from standard W3C vocabularies can be found https://pink-project.github.io/PINK-annotation-schema/widoco-reused-terms/index-en.html.
"""@en ;
    dcterms:bibliographicCitation "xxx" ;
    dcterms:contributor <https://orcid.org/0000-0003-4250-4584> ;
    dcterms:created "2025-09-08" ;
    dcterms:creator <https://orcid.org/0000-0002-1560-809X> ,
                    <https://orcid.org/0000-0001-8869-3718> ,
                    <https://orcid.org/0000-0002-1849-5246> ,
                    <https://orcid.org/0000-0002-8053-8198> ;
    dcterms:hasFormat <https://www.w3.org/TR/turtle/> ;
    #dcterms:issued "xxxx-xx-xxT00:00:00"^^xsd:dateTime ;
    dcterms:license "https://creativecommons.org/licenses/by/4.0/legalcode" ;
    #dcterms:modified "xxxx-xx-xxT00:00:00"^^xsd:dateTime ;
    dcterms:publisher <https://pink-project.eu/> ;
    #dcterms:source "Relevant PINK deliverable" ;
    dcterms:title "PINK Annotation Schema"@en ;
    bibo:doi "tbd" ;
    bibo:status <http://purl.org/ontology/bibo/status/forthcoming> ;
    vann:preferredNamespacePrefix "pink" ;
    vann:preferredNamespaceUri "https://w3id.org/pink" ;
    owl:priorVersion "0.0.0" ;
    owl:versionInfo "0.0.1" ;
    foaf:homepage <https://github.com/PINK-project/PINK-annotation-schema> ;
    foaf:logo <https://tess.elixir-europe.org/system/content_providers/images/000/000/777/original/pink-logo-orange-colorB-500.png> ;
    widoco:introduction """
The PINK Annotation Schema has a modular structure and aims to cover the following features:

* Allow to categorise resources (datasets, models, software, etc) according to their SSbD dimensions and categories/sub-categories.
* Provenance, based on the [PROV-O](https://www.w3.org/TR/prov-o/) ontology. PROV-O is fully adapted by the PINK Annotation Schema, having the three top-level PROV-O classes, *Activity*, *Entity* and *Agent* in root.
* Extension of the basic PROV-O provenance to complex scientific workflows with spatial and temporal parts.
* Allow documentation of workflows that have not (yet) been executed. Such documentation is done at class-level. When executed individuals should be created for the evaluated activities and their input and output providing a full PROV-O provenance graph.
* Top-level taxonomy for (advanced) materials and chemicals based on [EMMO](https://emmc.eu/emmo/) with mappings to [ChEBI](https://www.ebi.ac.uk/chebi/) for chemicals.
* Categorisation models.
* Strong taxonomy for relations, which are grouped into:
  - [parthood relations](https://pink-project.github.io/PINK-annotation-schema/docs/background.html#parthood-relations), based on mereology
  - [causal relations](https://pink-project.github.io/PINK-annotation-schema/docs/background.html#causal-relations), based on causality
  - [semiotic relations](https://pink-project.github.io/PINK-annotation-schema/docs/background.html#semiotic-relations), based on [Pierse semiotics](https://plato.stanford.edu/entries/peirce-semiotics/)

Separate reference documentations exists for the following sub-modules:

* [ddoc](https://pink-project.github.io/PINK-annotation-schema/widoco-ddoc/index-en.html): The Tripper data documentation vocabulary, with terms reused from other ontologies and vocabularies. Mainly [Dublin Core](https://www.dublincore.org/specifications/dublin-core/dcmi-terms/), [FOAF](http://xmlns.com/foaf/spec/) and similar basic vocabularies.
* [reused-terms](https://pink-project.github.io/PINK-annotation-schema/widoco-reused-terms/index-en.html): Additional reused terms by the PINK Annotation Schema ([DCAT](https://www.w3.org/TR/vocab-dcat-3/), [PROV-O](https://www.w3.org/TR/prov-o/), etc).
* [matter](https://pink-project.github.io/PINK-annotation-schema/widoco-matter/index-en.html): Taxonomy for (advanced) materials and chemicals
* [models](https://pink-project.github.io/PINK-annotation-schema/widoco-models/index-en.html): Taxonomy for models.

The root of the PINK Annotation Schema is shown below. More information can be found in the [background](https://pink-project.github.io/PINK-annotation-schema/docs/background.html) section.

"""@en .


## Contributors
<https://orcid.org/0000-0002-1560-809X> a foaf:Person ;
    skos:prefLabel "JesperFriis" ;
    foaf:name "Jesper Friis" ;
    foaf:workplaceHomepage <https://www.sintef.no/en/> .

<https://orcid.org/0000-0001-8869-3718> a foaf:Person ;
    skos:prefLabel "FrancescaLonstadBleken" ;
    foaf:name "Francesca Lønstad Bleken" ;
    foaf:workplaceHomepage <https://www.sintef.no/en/> .

<https://orcid.org/0000-0002-1849-5246> a foaf:Person ;
    skos:prefLabel "ThomasExner" ;
    foaf:name "Thomas Exner" ;
    foaf:workplaceHomepage <https://sevenpastnine.com/> .

<https://orcid.org/0000-0002-8053-8198> a foaf:Person ;
    skos:prefLabel "JohDokler" ;
    foaf:name "Joh Dokler" ;
    foaf:workplaceHomepage <https://sevenpastnine.com/> .

<https://orcid.org/0000-0003-4250-4584> a foaf:Person ;
    skos:prefLabel "IseultLynch" ;
    foaf:name "Iseult Lynch" ;
    foaf:workplaceHomepage <https://www.birmingham.ac.uk/> .



#################################################################
#    Annotation properties
#################################################################


###  http://purl.org/ontology/bibo/doi
bibo:doi rdf:type owl:AnnotationProperty .


###  http://purl.org/vocab/vann/preferredNamespacePrefix
vann:preferredNamespacePrefix rdf:type owl:AnnotationProperty .


###  http://purl.org/vocab/vann/preferredNamespaceUri
vann:preferredNamespaceUri rdf:type owl:AnnotationProperty .


###  http://xmlns.com/foaf/0.1/homepage
foaf:homepage rdf:type owl:AnnotationProperty .


###  http://xmlns.com/foaf/0.1/logo
foaf:logo rdf:type owl:AnnotationProperty .


skos:prefLabel rdf:type owl:AnnotationProperty .
skos:altLabel rdf:type owl:AnnotationProperty .
skos:definition rdf:type owl:AnnotationProperty .
skos:example rdf:type owl:AnnotationProperty .
skos:scopeNote rdf:type owl:AnnotationProperty .
vann:usageNote rdf:type owl:AnnotationProperty .


#################################################################
#    Data properties
#################################################################

:hasDataValue rdf:type owl:DatatypeProperty ;
    rdfs:domain :Data ;
    skos:prefLabel "hasDataValue"@en ;
    skos:definition "Relates a data individual to its literal value."@en .

:hasAPI a owl:DatatypeProperty ;
    rdfs:domain :Software ;
    rdfs:range xsd:boolean ;
    skos:prefLabel "hasAPI"@en ;
    skos:definition "Whether the software has an API." .

:hasGUI a owl:DatatypeProperty ;
    rdfs:domain :Software ;
    rdfs:range xsd:boolean ;
    skos:prefLabel "hasGUI"@en ;
    skos:definition "Whether the software has a GUI." .


#################################################################
#    Object properties
#################################################################

### SSbD relations

# TODO: Add rdfs:subPropertyOf
:ssbdDimension rdf:type owl:ObjectProperty ;
    rdfs:range :SsbdDimension ;
    skos:prefLabel "ssbdDimension"@en ;
    skos:definition "Note this class redefined in PR https://github.com/PINK-project/PINK-annotation-schema/pull/15"@en ;
    vann:usageNote "One of `pink:functionality`, `pink:safety`, `pink:environmental_sustainability`, `pink:social_sustainability`"@en .

:ssbdSubDimension rdf:type owl:DatatypeProperty ;
    rdfs:range xsd:string ;
    skos:prefLabel "ssbdSubDimension"@en ;
    skos:definition "Note this class redefined in PR https://github.com/PINK-project/PINK-annotation-schema/pull/15"@en .

:tierLevel a owl:ObjectProperty ;
    skos:prefLabel "tierLevel"@en ;
    rdfs:domain prov:Entity ;
    rdfs:range :TierLevel ;
    skos:definition "Relate an entity to an SSbD tier level."@en ;
    vann:usageNote "One of `pink:tierlevel1` (ideation/design), `pink:tierlevel2` (lab phase/development), `pink:tierlevel3` (up-scaling/production)"@en .

:chemicalClass rdf:type owl:ObjectProperty ;
    rdfs:domain prov:Entity ;
    rdfs:range pink:Matter ;
    skos:prefLabel "chemicalClass"@en ;
    skos:definition "Group of chemicals that and entity is relevant for."@en ;
    vann:usageNote "Choose one of subclasses of pink:Matter."@en .



### Other PINK-specific relations
:documentation a owl:ObjectProperty ;
    rdfs:subPropertyOf foaf:page;
    rdfs:domain dcat:Resource ;
    rdfs:range foaf:Document ;
    skos:prefLabel "documentation"@en ;
    skos:definition "A page or document documenting this resource." .


### Parthood relations
:overlaps rdf:type owl:ObjectProperty, owl:SymmetricProperty, owl:ReflexiveProperty ;
    skos:prefLabel "overlaps"@en ;
    owl:propertyDisjointWith :nonOverlaps ;
    skos:definition "The relation between two individuals representing entities that share at least one of their parts."@en .

:nonOverlaps rdf:type owl:ObjectProperty, owl:SymmetricProperty, owl:IrreflexiveProperty ;
    skos:prefLabel "nonOverlaps"@en ;
    owl:propertyDisjointWith :overlaps ;
    skos:definition "The relation between two individuals that does not share any parts."@en .

:isOvercrossedBy rdf:type owl:ObjectProperty, owl:IrreflexiveProperty ;
    rdfs:subPropertyOf :overlaps ;
    skos:prefLabel "isOvercrossedBy"@en ;
    owl:propertyDisjointWith :hasPart ;
    skos:definition "The relation between an entity that overlaps another without having it as part."@en .

:hasPart rdf:type owl:ObjectProperty, owl:ReflexiveProperty ;
    rdfs:subPropertyOf dcterms:hasPart, :overlaps ;
    skos:prefLabel "hasPart"@en ;
    skos:scopeNote "OWL2 does not allow non-simple (e.g. transitive) properties to appear in disjoint property axioms. We therefore implement the transitivity of hasPart using SWRL rules instead of asserting it with owl:TransitiveProperty."@en ;
    skos:definition "The primitive relation that express the concept of an entity being part of another one."@en .

:hasParticipant rdf:type owl:ObjectProperty, owl:IrreflexiveProperty, owl:AsymmetricProperty ;
    rdfs:subPropertyOf :hasPart ;
    skos:prefLabel "hasParticipant"@en ;
    skos:definition "The relation between a process and an object participating to it, i.e. that is relevant to the process itself."@en ;
    skos:scopeNote "Participation is a parthood relation - you must be part of the process to contribute to it. A participant whose 4D extension is totally contained within the process."@en .

:hasDatum rdf:type owl:ObjectProperty, owl:IrreflexiveProperty, owl:AsymmetricProperty ;
    rdfs:subPropertyOf :hasPart ;
    skos:prefLabel "hasDatum"@en ;
    rdfs:domain :Dataset ;
    rdfs:range :Datum ;
    skos:definition "Relates a dataset to its datum."@en .

:hasSpatialPart rdf:type owl:ObjectProperty, owl:IrreflexiveProperty, owl:AsymmetricProperty ;
    rdfs:subPropertyOf :hasPart ;
    skos:prefLabel "hasSpatialPart"@en ;
    skos:definition "A proper part of a whole, whose parts always cover the full temporal extension of the whole within a spatial interval."@en ;
    skos:scopeNote "The part is connected with the rest item or members with hasContact relations only (no hasNext)."@en .

:hasTemporalPart rdf:type owl:ObjectProperty, owl:IrreflexiveProperty, owl:AsymmetricProperty ;
    rdfs:subPropertyOf :hasPart ;
    skos:prefLabel "hasTemporalPart"@en ;
    skos:definition "A relation that identify a proper item part of the whole, whose parts always cover the full spatial extension of the whole within a time interval." ;
    skos:scopeNote "A temporal part of an item cannot both cause and be caused by any other proper part of the item."@en .

:hasJunctionPart rdf:type owl:ObjectProperty, owl:IrreflexiveProperty, owl:AsymmetricProperty ;
    rdfs:subPropertyOf :hasPart ;
    skos:prefLabel "hasJunctionPart"@en ;
    skos:altLabel "hasSpatioTemporalPart"@en ;
    skos:definition "The part is connected with the rest item or members with both hasNext (or its inverse) and hasContact relations."@en .


:participatesTo rdf:type owl:ObjectProperty, owl:IrreflexiveProperty, owl:AsymmetricProperty ;
    rdfs:subPropertyOf :isOvercrossedBy ;
    skos:prefLabel "participatesTo"@en ;
    rdfs:domain prov:Entity ;
    rdfs:range prov:Activity ;
    skos:scopeNote "The entity through overlaps the activity."@en ;
    skos:definition "Relation an entity to an activity that it interacts with."@en .

:used rdf:type owl:ObjectProperty, owl:IrreflexiveProperty, owl:AsymmetricProperty ;
    rdfs:subPropertyOf prov:used, :isOvercrossedBy ;
    skos:prefLabel "used"@en ;
    rdfs:domain prov:Activity ;
    rdfs:range prov:Entity ;
    skos:scopeNote "The activity A proper overlaps the entity E, where the non-overlapping part of E causes A."@en ;
    skos:definition "Relates an activity to an entity that it used."@en ;
    skos:example "For example, :baking :used :spoon, :egg, :oven ." .

:wasGeneratedBy rdf:type owl:ObjectProperty, owl:IrreflexiveProperty, owl:AsymmetricProperty ;
    rdfs:subPropertyOf prov:wasGeneratedBy, :isOvercrossedBy ;
    skos:prefLabel "wasGeneratedBy"@en ;
    rdfs:domain prov:Entity ;
    rdfs:range prov:Activity ;
    skos:scopeNote "The activity A proper overlaps the entity E, where the non-overlapping part of E is caused by A."@en ;
    skos:definition "Relates an entity to the activity it was generated from."@en .

:hasInput rdf:type owl:ObjectProperty, owl:IrreflexiveProperty, owl:AsymmetricProperty ;
    rdfs:subPropertyOf :used ;
    skos:prefLabel "hasInput"@en ;
    rdfs:domain prov:Activity ;
    rdfs:range prov:Entity ;
    skos:scopeNote "The activity A proper overlaps the entity E, where the non-overlapping part of E causes A."@en ;
    skos:definition "Relates an activity to an entity that is input to the activity."@en .

:hasOutput rdf:type owl:ObjectProperty, owl:IrreflexiveProperty, owl:AsymmetricProperty ;
    rdfs:subPropertyOf [ owl:inverseOf :wasGeneratedBy ] ;
    skos:prefLabel "hasOutput"@en ;
    rdfs:domain prov:Activity ;
    rdfs:range prov:Entity ;
    skos:scopeNote "The activity A proper overlaps the entity E, where the non-overlapping part of E is caused by A."@en ;
    skos:definition "Relates an activity to an entity that is the output of the activity."@en .

:wasAssociatedWith rdf:type owl:ObjectProperty, owl:IrreflexiveProperty, owl:AsymmetricProperty ;
    rdfs:subPropertyOf prov:wasAssociatedWith, :isOvercrossedBy ;
    skos:prefLabel "wasAssociatedWith"@en ;
    rdfs:domain prov:Activity ;
    rdfs:range prov:Agent ;
    skos:scopeNote "The activity is through overlapped by the agent."@en ;
    skos:definition "Relates an activity to an agent that had some (unspecified) responsibility for the occurence of this activity."@en .

:hasSoftware rdf:type owl:ObjectProperty, owl:IrreflexiveProperty, owl:AsymmetricProperty ;
    rdfs:subPropertyOf :wasAssociatedWith ;
    skos:prefLabel "hasSoftware"@en ;
    rdfs:domain :Computation ;
    rdfs:range :Software ;
    skos:definition "Relates a computation to the software used to perform the computation."@en .

:hasSubProcess rdf:type owl:ObjectProperty, owl:IrreflexiveProperty, owl:AsymmetricProperty ;
    rdfs:subPropertyOf :hasPart ;
    skos:prefLabel "hasSubProcess"@en ;
    rdfs:domain :Process ;
    rdfs:range :Process ;
    skos:definition "The relation between a process and one of its process parts."@en .

:assesses rdf:type owl:ObjectProperty, owl:IrreflexiveProperty, owl:AsymmetricProperty ;
    rdfs:subPropertyOf :isOvercrossedBy ;
    skos:prefLabel "assesses"@en ;
    rdfs:domain :Assessment ;
    rdfs:range :SsbdDimension ;
    skos:definition "Relates an assessment to a SSbD dimension."@en .

### Causal relations
:causedBy rdf:type owl:ObjectProperty, owl:IrreflexiveProperty ;
    rdfs:subPropertyOf prov:wasInfluencedBy ;
    skos:prefLabel "causedBy"@en ;
    skos:definition "A relation between an entity that causally affects the subject."@en ;
    skos:example "John yesterday is the cause of John today, is an example of temporal-like causality. The desk supporting my laptop is a space-like causality."@en .

:isAfter rdf:type owl:ObjectProperty, owl:IrreflexiveProperty, owl:AsymmetricProperty ;
    rdfs:subPropertyOf :causedBy ;
    skos:prefLabel "isAfter"@en ;
    skos:definition "A one-directional relation between an entity that affects the subject."@en .

:processedFrom rdf:type owl:ObjectProperty, owl:IrreflexiveProperty, owl:AsymmetricProperty ;
    rdfs:subPropertyOf :isAfter ;
    skos:prefLabel "processedFrom"@en ;
    skos:definition "Indirect relation that relates the output of an activity to its input."@en .

:wasInformedBy rdf:type owl:ObjectProperty, owl:IrreflexiveProperty, owl:AsymmetricProperty ;
    rdfs:subPropertyOf :isAfter, prov:wasInformedBy ;
    skos:prefLabel "wasInformedBy"@en ;
    skos:definition "A one-directional relation between an activity that affects the subject activity."@en ;
    rdfs:domain prov:Activity ;
    rdfs:range prov:Activity .

:wasDerivedBy rdf:type owl:ObjectProperty, owl:IrreflexiveProperty, owl:AsymmetricProperty ;
    rdfs:subPropertyOf :processedFrom, prov:wasDerivedBy ;
    skos:prefLabel "wasDerivedBy"@en ;
    skos:definition "Indirect relation that relates the output entity of an activity to its input entity."@en ;
    rdfs:domain prov:Entity ;
    rdfs:range prov:Entity .

:wasAttributedTo rdf:type owl:ObjectProperty, owl:IrreflexiveProperty, owl:AsymmetricProperty ;
    rdfs:subPropertyOf prov:wasAttributedTo, :causedBy ;
    skos:prefLabel "wasAttributedTo"@en ;
    rdfs:domain prov:Entity ;
    rdfs:range prov:Agent ;
    skos:definition "Relates an entity to an agent via an activity that both the entity and agent participates to."@en ;
    skos:scopeNote "The activity is through overlapped by the agent and overcrossed by the entity."@en ;
    owl:inverseOf :attributed .

:attributed rdf:type owl:ObjectProperty, owl:IrreflexiveProperty, owl:AsymmetricProperty ;
    rdfs:subPropertyOf :causedBy ;
    skos:prefLabel "attributed"@en ;
    rdfs:domain prov:Agent ;
    rdfs:range prov:Entity ;
    skos:definition "Relates an agent to an entity via an activity that both the agent and entity participates to."@en ;
    skos:scopeNote "There may or may not be a causal interaction between the agent and entity."@en ;
    skos:scopeNote "The activity is through overlapped by the agent and overcrossed by the entity."@en ;
    owl:inverseOf :wasAttributedTo .

:priorRelease rdf:type owl:ObjectProperty, owl:IrreflexiveProperty, owl:AsymmetricProperty ;
    rdfs:subPropertyOf :causedBy ;
    skos:prefLabel "priorRelease"@en ;
    rdfs:domain :Software ;
    rdfs:range :Software ;
    skos:definition "Direct relation that relates a software to the most resent earlier release of the software."@en ;
    skos:scopeNote "Useful for tracking the provenance of software releases."@en .


### Semiotic relations
:semiotical rdf:type owl:ObjectProperty ;
    skos:prefLabel "semiotical"@en ;
    skos:definition "The base of all semiotic relations."@en ;
    skos:scopeNote "Semiotic relations take part in a triadic semiotic meaning-making process, where an 'interpreter' connects a 'sign' (e.g. a property) to an entity (called 'referent')."@en ;
    skos:scopeNote "The semiotic relations in the PINK Annotation Scheme are inspirred by EMMO, which in turn is based on the semiotic theory by Charles Sanders Peirce (1839-1914)."@en ;
    skos:scopeNote "Semiotic relations can be seen as shortcuts that replaces a series of complex causal relations with a single relation."@en .

:isInterpretedBy rdf:type owl:ObjectProperty ;
    rdfs:subPropertyOf :semiotical ;
    skos:prefLabel "isInterpretedBy"@en ;
    skos:definition "Connects a sign (e.g. a property) to an interpreter."@en ;
    rdfs:domain :Sign ;
    rdfs:range :Interpreter .

:isRepresentedBy rdf:type owl:ObjectProperty ;
    rdfs:subPropertyOf :semiotical ;
    owl:inverseOf :standsFor ;
    skos:prefLabel "isRepresentedBy"@en ;
    skos:definition "Connects an entity to a sign that stands for the entity."@en ;
    rdfs:domain prov:Entity ;
    rdfs:range :Sign .

:hasProperty rdf:type owl:ObjectProperty ;
    rdfs:subPropertyOf :isRepresentedBy ;
    skos:prefLabel "hasProperty"@en ;
    skos:definition "Connects a thing to one of its properties."@en ;
    rdfs:range :Property .

:hasDescription rdf:type owl:ObjectProperty ;
    rdfs:subPropertyOf :isRepresentedBy ;
    skos:prefLabel "hasDescription"@en ;
    skos:definition "Connects a thing to a description (i.e. collection of properties) of the thing."@en ;
    rdfs:range :Description .

:hasUnit rdf:type owl:ObjectProperty ;
    rdfs:subPropertyOf :hasDescription ;
    skos:prefLabel "hasUnit"@en ;
    skos:definition "Connects a property to its unit."@en ;
    skos:scopeNote "`pink:hasUnit` is intended to refer to a unit in an existing unit ontology, like QUDT or EMMO."@en ;
    vann:usageNote """A universal restriction should be used when referring to a unit in EMMO.  For example:

    :LethalDose50
        a pink:Toxicity , [
            a owl:Restriction ;
            owl:onProperty pink:hasUnit ;
            owl:someValuesFrom emmo:MilliGramPerKiloGram
        ] .
"""@en ;
    rdfs:domain :Property .

:standsFor rdf:type owl:ObjectProperty ;
    rdfs:subPropertyOf :semiotical ;
    owl:inverseOf :isRepresentedBy ;
    skos:prefLabel "standsFor"@en ;
    skos:definition "Connects a sign (e.g. a property) to an entity (a 'referent')."@en ;
    rdfs:domain :Sign ;
    rdfs:range prov:Entity .

:isDescriptionOf rdf:type owl:ObjectProperty ;
    rdfs:subPropertyOf :standsFor ;
    owl:inverseOf :hasDescription ;
    skos:prefLabel "isDescriptionOf"@en ;
    skos:definition "Connects a description to an entity."@en ;
    rdfs:domain :Description ;
    rdfs:range prov:Entity .

:isPropertyOf rdf:type owl:ObjectProperty ;
    rdfs:subPropertyOf :standsFor ;
    owl:inverseOf :hasProperty ;
    skos:prefLabel "isPropertyOf"@en ;
    skos:definition "Connects a property to an entity."@en ;
    rdfs:domain :Property ;
    rdfs:range prov:Entity .

:implementsModel rdf:type owl:ObjectProperty, owl:IrreflexiveProperty, owl:AsymmetricProperty ;
    rdfs:subPropertyOf :standsFor ;
    skos:prefLabel "implementsModel"@en ;
    rdfs:domain :Software ;
    rdfs:range :Model ;
    skos:definition "Relates a software to the model it implements."@en ;
    skos:scopeNote "Semiotically a software can be seen as an executable sign that stands for the model it implements."@en .



#################################################################
#    Classes
#################################################################

### Activity subclasses
:Process rdf:type owl:Class ;
    rdfs:subClassOf prov:Activity ;
    skos:prefLabel "Process"@en ;
    skos:altLabel "Occurent"@en ;
    skos:altLabel "Perdurant"@en ;
    skos:definition "An activity with temporal parts."@en ;
    skos:scopeNote "The temporal parts of a process are not of the same type as the process itself."@en .

:MaterialProcess rdf:type owl:Class ;
    rdfs:subClassOf :Process ;
    skos:prefLabel "MaterialProcess"@en ;
    skos:definition "A process that has material as input and output."@en .

:Measurement rdf:type owl:Class ;
    rdfs:subClassOf :Process ;
    skos:prefLabel "Measurement"@en ;
    skos:definition "An observation that results in a quantitative comparison of a 'property' of an 'object' with a standard reference based on a well defined mesurement procedure."@en .

:Computation rdf:type owl:Class ;
    rdfs:subClassOf :Process ;
    skos:prefLabel "Computation"@en ;
    skos:definition "A process that deals with quantitative symbols (i.e. symbols associated with a quantitative oriented language)."@en .


### Entity subclasses
:Matter rdf:type owl:Class ;
    rdfs:subClassOf prov:Entity ;
    skos:prefLabel "Matter"@en ;
    skos:definition "An entity that possess mass and occupies volume."@en ;
    skos:scopeNote "From the definition it follows that matter is an object with fermionic parts."@en ,
     """The interpretation of the term "matter" is not univocal. Several concepts are labelled with this term, depending on the field of science. The concept mass is sometimes related to the term "matter", even if the former refers to a physical quantity (precisely defined by modern physics) while the latter is a type that qualifies a physical entity.
It is possible to identify more than one concept that can be reasonably labelled with the term "matter". For example, it is possible to label as matter only the entities that are made up of atoms. Or more generally, we can be more fine-grained and call "matter" the entities that are made up of protons, neutrons or electrons, so that we can call matter also a neutron radiation or a cathode ray.
A more fundamental approach taken here, considers matter as entities that are made of quarks and leptons, without excluding particles like the W and Z bosons that possess some mass, but are not fermions. This definition also include antimatter."""@en .

emmo:Substance rdfs:subClassOf :Matter .
emmo:ChemicalEntity rdfs:subClassOf :Matter .


## Data
:Data rdf:type owl:Class ;
    rdfs:subClassOf prov:Entity ;
    skos:prefLabel "Data"@en ;
    skos:definition "Contrast from variation of properties that is encoded by an agent and that can be decoded by another agent according to a specific rule."@en .

:Software rdf:type owl:Class ;
    rdfs:subClassOf :Data ;
    skos:prefLabel "Software"@en ;
    skos:definition "All or part of the programs, procedures, rules, and associated documentation of an information processing system."@en .

:ComputationalTool rdf:type owl:Class ;
    rdfs:subClassOf :Software ;
    skos:prefLabel "ComputationalTool"@en ;
    skos:definition "A software that performs a computation."@en ;
    skos:example "Gromacs is a computational tool that solves Newton's equations of motion."@en .

:Datum rdf:type owl:Class ;
    rdfs:subClassOf :Data ;
    skos:prefLabel "Datum"@en ;
    skos:definition "A self-consistent encoded data entity."@en ;
    vann:usageNote "Datum is the building block of datasets."@en .

:Dataset rdf:type owl:Class ;
    rdfs:subClassOf :Data, [
        rdf:type owl:Restriction ;
        owl:onProperty :hasPart ;
        owl:someValuesFrom :Datum
    ] ;
    skos:prefLabel "Dataset"@en ;
    skos:definition "Encoded data made of more than one datum."@en ;
    vann:usageNote "A collection of (more than one) datum, published or curated by a single agent, and available for access or download in one or more representations."@en .

:ReliabilityDocument rdf:type owl:Class ;
    rdfs:subClassOf foaf:Document ;
    skos:prefLabel "ReliabilityDocument"@en ;
    skos:definition "xxx"@en ;
    vann:usageNote "xxx"@en .


:SymbolicData rdf:type owl:Class ;
    rdfs:subClassOf :Data ;
    rdfs:seeAlso <https://www.w3.org/TR/2012/REC-owl2-syntax-20121211/#Datatype_Maps> ;
    rdfs:seeAlso <https://www.w3.org/TR/2012/REC-xmlschema11-2-20120405/#built-in-datatypes> ;
    skos:prefLabel "SymbolicData"@en ;
    skos:definition "The class for entities which stands for a specific data format expressed using a symbolic encoding."@en .

:NumericalData rdf:type owl:Class ;
    rdfs:subClassOf :SymbolicData ;
    skos:prefLabel "NumericalData"@en ;
    skos:definition "A symbolic data representing a numerical value."@en .

:FloatData rdf:type owl:Class ;
    rdfs:subClassOf :NumericalData ;
    rdfs:seeAlso <https://www.w3.org/TR/xmlschema11-2/#float> ;
    skos:prefLabel "FloatData"@en ;
    skos:definition "A symbolic data representing a 32-bit floating point numbers incl. ±Inf, ±0, NaN."@en .

:DoubleData rdf:type owl:Class ;
    rdfs:subClassOf :NumericalData ;
    rdfs:seeAlso <https://www.w3.org/TR/xmlschema11-2/#double> ;
    skos:prefLabel "DoubleData"@en ;
    skos:definition "A symbolic data representing a 64-bit floating point numbers incl. ±Inf, ±0, NaN."@en .

:IntegerData rdf:type owl:Class ;
    rdfs:subClassOf :NumericalData ;
    rdfs:seeAlso <https://www.w3.org/TR/xmlschema11-2/#integer> ;
    skos:prefLabel "IntegerData"@en ;
    skos:definition "A data representing an arbritrary sized integer number."@en .

:LongData rdf:type owl:Class ;
    rdfs:subClassOf :IntegerData ;
    rdfs:seeAlso <https://www.w3.org/TR/xmlschema11-2/#long> ;
    skos:prefLabel "LongData"@en ;
    skos:definition "A data representing a 64-bit integer number."@en .

:IntData rdf:type owl:Class ;
    rdfs:subClassOf :LongData ;
    rdfs:seeAlso <https://www.w3.org/TR/xmlschema11-2/#int> ;
    skos:prefLabel "IntData"@en ;
    skos:definition "A data representing a 32-bit integer number."@en .

:ShortData rdf:type owl:Class ;
    rdfs:subClassOf :IntData ;
    rdfs:seeAlso <https://www.w3.org/TR/xmlschema11-2/#short> ;
    skos:prefLabel "ShortData"@en ;
    skos:definition "A data representing a 16-bit integer number."@en .

:ByteData rdf:type owl:Class ;
    rdfs:subClassOf :ShortData ;
    rdfs:seeAlso <https://www.w3.org/TR/xmlschema11-2/#byte> ;
    skos:prefLabel "ByteData"@en ;
    skos:definition "A data representing a 8-bit integer number."@en .

:BooleanData rdf:type owl:Class ;
    rdfs:subClassOf :SymbolicData ;
    rdfs:seeAlso <https://www.w3.org/TR/xmlschema11-2/#boolean> ;
    skos:prefLabel "BooleanData"@en ;
    skos:definition "A symbolic data representing a boolean number."@en .

:DateData rdf:type owl:Class ;
    rdfs:subClassOf :SymbolicData ;
    rdfs:seeAlso <https://www.w3.org/TR/xmlschema11-2/#date> ;
    skos:prefLabel "DateData"@en ;
    skos:definition "A symbolic data representing date. Format: YYYY-MM-DD (followed by an optional time zone offset, e.g. +01:00 for Central Europe)."@en .

:TimeData rdf:type owl:Class ;
    rdfs:subClassOf :SymbolicData ;
    rdfs:seeAlso <https://www.w3.org/TR/xmlschema11-2/#time> ;
    skos:prefLabel "TimeData"@en ;
    skos:definition "A symbolic data representing time. Format: hh:mm:ss (followed by an optional time zone offset, e.g. +01:00 for Central Europe)."@en .

:DateTimeData rdf:type owl:Class ;
    rdfs:subClassOf :SymbolicData ;
    rdfs:seeAlso <https://www.w3.org/TR/xmlschema11-2/#dateTime> ;
    skos:prefLabel "DateTimeData"@en ;
    skos:definition "A symbolic data representing datetime. Format: YYYY-MM-DDThh:mm:ss (followed by an optional time zone offset, e.g. +01:00 for Central Europe)."@en .



## Sign
:Sign rdf:type owl:Class ;
    rdfs:subClassOf prov:Entity ;
    skos:prefLabel "Sign"@en ;
    skos:definition "A sign that stands for an entity."@en ;
    skos:scopeNote "A sign is a part of a triadic semiotic (meaning-making) process, where an 'interpreter' connects a 'sign' to an entity (called 'referent')."@en .

:Information rdf:type owl:Class ;
    rdfs:subClassOf :Sign, :Data ;
    skos:prefLabel "Information"@en ;
    skos:Definition "Data with meaning (semiotic sign)."@en ;
    rdfs:isDefinedBy "Luciano Floridi, Information - A Very Short Introduction, Oxford University Press (2010) ISBN: 9780199551378"@en .

:Model rdf:type owl:Class ;
    rdfs:subClassOf :Sign ;
    skos:prefLabel "Model"@en ;
    skos:definition "A useful simplified description of a selected part of the world."@en ;
    skos:scopeNote "A model is a sign that resembles or imitates an object, in shape, function or by sharing a similar logical structure."@en ;
    skos:example """Newton's law of motion is a model for how a body will move when subjected to forces.
A mouse can be seen as a model for a human (e.g. in medicine).
An architectural floor plan is a model of a house.
"""@en .

:Property rdf:type owl:Class ;
    rdfs:subClassOf :Sign ;
    skos:prefLabel "Property"@en ;
    skos:definition """An "atomic" sign that stands for an physical interaction with an object."""@en ;
    skos:scopeNote "A property is atomic in the sense that is aimed to deliver one and one only aspect of the object."@en .

:Indicator rdf:type owl:Class ;
    rdfs:subClassOf :Property ;
    skos:prefLabel "Indicator"@en ;
    skos:altLabel "Descriptor"@en ;
    skos:altLabel "EndPoint"@en ;
    skos:definition "A property that provides information about the state of a system. It simplifies complex realities into measurable values that can guide decisions."@en ;
    skos:example "For a computation is an indicator a specific property/datum that is provided in the output."@en .


:Toxicity rdf:type owl:Class ;
    rdfs:subClassOf :Sign ;
    skos:prefLabel "Toxicity"@en ;
    skos:definition "The property or ability of a substance to cause harmful health effects."@en ;
    skos:scopeNote "The helth effects can strike a single cell, a group of cells, an organ system, or the entire body. A toxic effect may be visible damage, or a decrease in performance or function measurable only by a test."@en ;
    skos:scopeNote "Toxicity is always related to a given measurement procedure. Hence, the user is expected to define spesific subclasses defining the measurement procedure that the toxicity is measured according to."@en .

:Description rdf:type owl:Class ;
    rdfs:subClassOf :Sign ;
    skos:prefLabel "Description"@en ;
    skos:definition "A collection of properties that depicts an object."@en ;
    skos:scopeNote "A description is not atomic in the sense that it is made of more than one property."@en .

## Object
:Object rdf:type owl:Class ;
    rdfs:subClassOf prov:Entity ;
    skos:prefLabel "Object"@en ;
    skos:altLabel "Continuant"@en ;
    skos:altLabel "Endurant"@en ;
    skos:definition "An entity that has a temporal extension."@en ;
    skos:scopeNote "Object is the class of all individuals who's temporal parts are of the same type as the whole."@en ;
    skos:scopeNote "Object individals will typically also be an individual of 'Matter'. However, when categorising something as an 'Object', the focus is on its existence (throughout one of more processes), while 'Matter' focuses on that it pocess mass and takes up volume and how it can further be categorised as "@en .


## Tier level
:TierLevel rdf:type owl:Class ;
    rdfs:subClassOf prov:Entity ;
    skos:prefLabel "TierLevel"@en ;
    skos:definition "Represent a tiered, iterative framework for evaluating chemical and material safety from early innovation to production."@en ;
    skos:scopeNote "This approach typically involves a three-tier system-ranging from qualitative, early-stage, in silico, and in vitro screening to, finally, advanced, quantitative, in vivo testing."@en .


### Agent subclasses
:Participant rdf:type owl:Class ;
    rdfs:subClassOf :Object, prov:Agent ;
    skos:prefLabel "Participant"@en ;
    skos:definition "An object that participates to a process."@en ;
    skos:scopeNote "Mereologically participation means that the object is a spatial part of the process."@en ;
    skos:example "A student during an examination. The student exists both before and after the examination."@en .

:Interpreter rdf:type owl:Class ;
    rdfs:subClassOf prov:Agent ;
    skos:prefLabel "Interpreter"@en ;
    skos:definition "The agent that connects the sign to an entity in a semiotic (meaning-making) process."@en ;
    skos:example "A person (interpreter) that measures the length (sign) of an pencil (object)."@en .


### Mappings
### Include standard concepts into the PINK taxonomy
### Question: should we duplicate these classes instead?
foaf:Document rdfs:subClassOf :Data .
prov:Agent rdfs:subClassOf foaf:Agent .
dcat:Resource rdfs:subClassOf prov:Entity .
foaf:Organization rdfs:subClassOf :Object .
foaf:Person rdfs:subClassOf :Object .
foaf:Project rdfs:subClassOf prov:Entity .
dcterms:RightsStatement rdfs:subClassOf foaf:Document .
:SsbdDimension  rdfs:subClassOf prov:Entity .


#################################################################
#    Individuals
#################################################################

### TierLevel individuals
:tierlevel1 a :TierLevel ;
    rdfs:label "ideation/design"@en .

:tierlevel2 a :TierLevel ;
    rdfs:label "lab phase/development"@en .

:tierlevel3 a :TierLevel ;
    rdfs:label "up-scaling/production"@en .


#################################################################
#    Rules
#################################################################

<urn:swrl:var#x> rdf:type <http://www.w3.org/2003/11/swrl#Variable> .

<urn:swrl:var#y> rdf:type <http://www.w3.org/2003/11/swrl#Variable> .

<urn:swrl:var#z> rdf:type <http://www.w3.org/2003/11/swrl#Variable> .

[ rdf:type <http://www.w3.org/2003/11/swrl#Imp> ;
   <http://www.w3.org/2003/11/swrl#body> [ rdf:type <http://www.w3.org/2003/11/swrl#AtomList> ;
                                           rdf:first [ rdf:type <http://www.w3.org/2003/11/swrl#IndividualPropertyAtom> ;
                                                       <http://www.w3.org/2003/11/swrl#propertyPredicate> :hasProcess ;
                                                       <http://www.w3.org/2003/11/swrl#argument1> <urn:swrl:var#x> ;
                                                       <http://www.w3.org/2003/11/swrl#argument2> <urn:swrl:var#y>
                                                     ] ;
                                           rdf:rest [ rdf:type <http://www.w3.org/2003/11/swrl#AtomList> ;
                                                      rdf:first [ rdf:type <http://www.w3.org/2003/11/swrl#IndividualPropertyAtom> ;
                                                                  <http://www.w3.org/2003/11/swrl#propertyPredicate> :wasGeneratedBy ;
                                                                  <http://www.w3.org/2003/11/swrl#argument1> <urn:swrl:var#z> ;
                                                                  <http://www.w3.org/2003/11/swrl#argument2> <urn:swrl:var#y>
                                                                ] ;
                                                      rdf:rest rdf:nil
                                                    ]
                                         ] ;
   <http://www.w3.org/2003/11/swrl#head> [ rdf:type <http://www.w3.org/2003/11/swrl#AtomList> ;
                                           rdf:first [ rdf:type <http://www.w3.org/2003/11/swrl#IndividualPropertyAtom> ;
                                                       <http://www.w3.org/2003/11/swrl#propertyPredicate> :output ;
                                                       <http://www.w3.org/2003/11/swrl#argument1> <urn:swrl:var#x> ;
                                                       <http://www.w3.org/2003/11/swrl#argument2> <urn:swrl:var#z>
                                                     ] ;
                                           rdf:rest rdf:nil
                                         ]
 ] .

[ rdf:type <http://www.w3.org/2003/11/swrl#Imp> ;
   <http://www.w3.org/2003/11/swrl#body> [ rdf:type <http://www.w3.org/2003/11/swrl#AtomList> ;
                                           rdf:first [ rdf:type <http://www.w3.org/2003/11/swrl#IndividualPropertyAtom> ;
                                                       <http://www.w3.org/2003/11/swrl#propertyPredicate> :used ;
                                                       <http://www.w3.org/2003/11/swrl#argument1> <urn:swrl:var#x> ;
                                                       <http://www.w3.org/2003/11/swrl#argument2> <urn:swrl:var#y>
                                                     ] ;
                                           rdf:rest [ rdf:type <http://www.w3.org/2003/11/swrl#AtomList> ;
                                                      rdf:first [ rdf:type <http://www.w3.org/2003/11/swrl#IndividualPropertyAtom> ;
                                                                  <http://www.w3.org/2003/11/swrl#propertyPredicate> :wasGeneratedBy ;
                                                                  <http://www.w3.org/2003/11/swrl#argument1> <urn:swrl:var#y> ;
                                                                  <http://www.w3.org/2003/11/swrl#argument2> <urn:swrl:var#z>
                                                                ] ;
                                                      rdf:rest rdf:nil
                                                    ]
                                         ] ;
   <http://www.w3.org/2003/11/swrl#head> [ rdf:type <http://www.w3.org/2003/11/swrl#AtomList> ;
                                           rdf:first [ rdf:type <http://www.w3.org/2003/11/swrl#IndividualPropertyAtom> ;
                                                       <http://www.w3.org/2003/11/swrl#propertyPredicate> :wasInformedBy ;
                                                       <http://www.w3.org/2003/11/swrl#argument1> <urn:swrl:var#x> ;
                                                       <http://www.w3.org/2003/11/swrl#argument2> <urn:swrl:var#z>
                                                     ] ;
                                           rdf:rest rdf:nil
                                         ]
 ] .

[ rdf:type <http://www.w3.org/2003/11/swrl#Imp> ;
   <http://www.w3.org/2003/11/swrl#body> [ rdf:type <http://www.w3.org/2003/11/swrl#AtomList> ;
                                           rdf:first [ rdf:type <http://www.w3.org/2003/11/swrl#IndividualPropertyAtom> ;
                                                       <http://www.w3.org/2003/11/swrl#propertyPredicate> :wasAssociatedWith ;
                                                       <http://www.w3.org/2003/11/swrl#argument1> <urn:swrl:var#y> ;
                                                       <http://www.w3.org/2003/11/swrl#argument2> <urn:swrl:var#x>
                                                     ] ;
                                           rdf:rest [ rdf:type <http://www.w3.org/2003/11/swrl#AtomList> ;
                                                      rdf:first [ rdf:type <http://www.w3.org/2003/11/swrl#IndividualPropertyAtom> ;
                                                                  <http://www.w3.org/2003/11/swrl#propertyPredicate> :used ;
                                                                  <http://www.w3.org/2003/11/swrl#argument1> <urn:swrl:var#y> ;
                                                                  <http://www.w3.org/2003/11/swrl#argument2> <urn:swrl:var#z>
                                                                ] ;
                                                      rdf:rest rdf:nil
                                                    ]
                                         ] ;
   <http://www.w3.org/2003/11/swrl#head> [ rdf:type <http://www.w3.org/2003/11/swrl#AtomList> ;
                                           rdf:first [ rdf:type <http://www.w3.org/2003/11/swrl#IndividualPropertyAtom> ;
                                                       <http://www.w3.org/2003/11/swrl#propertyPredicate> :attributed ;
                                                       <http://www.w3.org/2003/11/swrl#argument1> <urn:swrl:var#x> ;
                                                       <http://www.w3.org/2003/11/swrl#argument2> <urn:swrl:var#z>
                                                     ] ;
                                           rdf:rest rdf:nil
                                         ]
 ] .

[ rdf:type <http://www.w3.org/2003/11/swrl#Imp> ;
   <http://www.w3.org/2003/11/swrl#body> [ rdf:type <http://www.w3.org/2003/11/swrl#AtomList> ;
                                           rdf:first [ rdf:type <http://www.w3.org/2003/11/swrl#IndividualPropertyAtom> ;
                                                       <http://www.w3.org/2003/11/swrl#propertyPredicate> :wasGeneratedBy ;
                                                       <http://www.w3.org/2003/11/swrl#argument1> <urn:swrl:var#x> ;
                                                       <http://www.w3.org/2003/11/swrl#argument2> <urn:swrl:var#y>
                                                     ] ;
                                           rdf:rest [ rdf:type <http://www.w3.org/2003/11/swrl#AtomList> ;
                                                      rdf:first [ rdf:type <http://www.w3.org/2003/11/swrl#IndividualPropertyAtom> ;
                                                                  <http://www.w3.org/2003/11/swrl#propertyPredicate> :used ;
                                                                  <http://www.w3.org/2003/11/swrl#argument1> <urn:swrl:var#y> ;
                                                                  <http://www.w3.org/2003/11/swrl#argument2> <urn:swrl:var#z>
                                                                ] ;
                                                      rdf:rest rdf:nil
                                                    ]
                                         ] ;
   <http://www.w3.org/2003/11/swrl#head> [ rdf:type <http://www.w3.org/2003/11/swrl#AtomList> ;
                                           rdf:first [ rdf:type <http://www.w3.org/2003/11/swrl#IndividualPropertyAtom> ;
                                                       <http://www.w3.org/2003/11/swrl#propertyPredicate> :processedFrom ;
                                                       <http://www.w3.org/2003/11/swrl#argument1> <urn:swrl:var#x> ;
                                                       <http://www.w3.org/2003/11/swrl#argument2> <urn:swrl:var#z>
                                                     ] ;
                                           rdf:rest rdf:nil
                                         ]
 ] .

[ rdf:type <http://www.w3.org/2003/11/swrl#Imp> ;
   <http://www.w3.org/2003/11/swrl#body> [ rdf:type <http://www.w3.org/2003/11/swrl#AtomList> ;
                                           rdf:first [ rdf:type <http://www.w3.org/2003/11/swrl#IndividualPropertyAtom> ;
                                                       <http://www.w3.org/2003/11/swrl#propertyPredicate> :wasGeneratedBy ;
                                                       <http://www.w3.org/2003/11/swrl#argument1> <urn:swrl:var#x> ;
                                                       <http://www.w3.org/2003/11/swrl#argument2> <urn:swrl:var#y>
                                                     ] ;
                                           rdf:rest [ rdf:type <http://www.w3.org/2003/11/swrl#AtomList> ;
                                                      rdf:first [ rdf:type <http://www.w3.org/2003/11/swrl#IndividualPropertyAtom> ;
                                                                  <http://www.w3.org/2003/11/swrl#propertyPredicate> :used ;
                                                                  <http://www.w3.org/2003/11/swrl#argument1> <urn:swrl:var#y> ;
                                                                  <http://www.w3.org/2003/11/swrl#argument2> <urn:swrl:var#z>
                                                                ] ;
                                                      rdf:rest rdf:nil
                                                    ]
                                         ] ;
   <http://www.w3.org/2003/11/swrl#head> [ rdf:type <http://www.w3.org/2003/11/swrl#AtomList> ;
                                           rdf:first [ rdf:type <http://www.w3.org/2003/11/swrl#IndividualPropertyAtom> ;
                                                       <http://www.w3.org/2003/11/swrl#propertyPredicate> :wasDerivedBy ;
                                                       <http://www.w3.org/2003/11/swrl#argument1> <urn:swrl:var#x> ;
                                                       <http://www.w3.org/2003/11/swrl#argument2> <urn:swrl:var#z>
                                                     ] ;
                                           rdf:rest rdf:nil
                                         ]
 ] .

[ rdf:type <http://www.w3.org/2003/11/swrl#Imp> ;
   <http://www.w3.org/2003/11/swrl#body> [ rdf:type <http://www.w3.org/2003/11/swrl#AtomList> ;
                                           rdf:first [ rdf:type <http://www.w3.org/2003/11/swrl#IndividualPropertyAtom> ;
                                                       <http://www.w3.org/2003/11/swrl#propertyPredicate> :hasProcess ;
                                                       <http://www.w3.org/2003/11/swrl#argument1> <urn:swrl:var#x> ;
                                                       <http://www.w3.org/2003/11/swrl#argument2> <urn:swrl:var#y>
                                                     ] ;
                                           rdf:rest [ rdf:type <http://www.w3.org/2003/11/swrl#AtomList> ;
                                                      rdf:first [ rdf:type <http://www.w3.org/2003/11/swrl#IndividualPropertyAtom> ;
                                                                  <http://www.w3.org/2003/11/swrl#propertyPredicate> :used ;
                                                                  <http://www.w3.org/2003/11/swrl#argument1> <urn:swrl:var#y> ;
                                                                  <http://www.w3.org/2003/11/swrl#argument2> <urn:swrl:var#z>
                                                                ] ;
                                                      rdf:rest rdf:nil
                                                    ]
                                         ] ;
   <http://www.w3.org/2003/11/swrl#head> [ rdf:type <http://www.w3.org/2003/11/swrl#AtomList> ;
                                           rdf:first [ rdf:type <http://www.w3.org/2003/11/swrl#IndividualPropertyAtom> ;
                                                       <http://www.w3.org/2003/11/swrl#propertyPredicate> :input ;
                                                       <http://www.w3.org/2003/11/swrl#argument1> <urn:swrl:var#x> ;
                                                       <http://www.w3.org/2003/11/swrl#argument2> <urn:swrl:var#z>
                                                     ] ;
                                           rdf:rest rdf:nil
                                         ]
 ] .

[ rdf:type <http://www.w3.org/2003/11/swrl#Imp> ;
   <http://www.w3.org/2003/11/swrl#body> [ rdf:type <http://www.w3.org/2003/11/swrl#AtomList> ;
                                           rdf:first [ rdf:type <http://www.w3.org/2003/11/swrl#IndividualPropertyAtom> ;
                                                       <http://www.w3.org/2003/11/swrl#propertyPredicate> pink:hasPart ;
                                                       <http://www.w3.org/2003/11/swrl#argument1> <urn:swrl:var#x> ;
                                                       <http://www.w3.org/2003/11/swrl#argument2> <urn:swrl:var#y>
                                                     ] ;
                                           rdf:rest [ rdf:type <http://www.w3.org/2003/11/swrl#AtomList> ;
                                                      rdf:first [ rdf:type <http://www.w3.org/2003/11/swrl#IndividualPropertyAtom> ;
                                                                  <http://www.w3.org/2003/11/swrl#propertyPredicate> pink:hasPart ;
                                                                  <http://www.w3.org/2003/11/swrl#argument1> <urn:swrl:var#y> ;
                                                                  <http://www.w3.org/2003/11/swrl#argument2> <urn:swrl:var#z>
                                                                ] ;
                                                      rdf:rest rdf:nil
                                                    ]
                                         ] ;
   <http://www.w3.org/2003/11/swrl#head> [ rdf:type <http://www.w3.org/2003/11/swrl#AtomList> ;
                                           rdf:first [ rdf:type <http://www.w3.org/2003/11/swrl#IndividualPropertyAtom> ;
                                                       <http://www.w3.org/2003/11/swrl#propertyPredicate> pink:hasPart ;
                                                       <http://www.w3.org/2003/11/swrl#argument1> <urn:swrl:var#x> ;
                                                       <http://www.w3.org/2003/11/swrl#argument2> <urn:swrl:var#z>
                                                     ] ;
                                           rdf:rest rdf:nil
                                         ]
 ] .

[ rdf:type <http://www.w3.org/2003/11/swrl#Imp> ;
   <http://www.w3.org/2003/11/swrl#body> [ rdf:type <http://www.w3.org/2003/11/swrl#AtomList> ;
                                           rdf:first [ rdf:type <http://www.w3.org/2003/11/swrl#IndividualPropertyAtom> ;
                                                       <http://www.w3.org/2003/11/swrl#propertyPredicate> :wasGeneratedBy ;
                                                       <http://www.w3.org/2003/11/swrl#argument1> <urn:swrl:var#x> ;
                                                       <http://www.w3.org/2003/11/swrl#argument2> <urn:swrl:var#y>
                                                     ] ;
                                           rdf:rest [ rdf:type <http://www.w3.org/2003/11/swrl#AtomList> ;
                                                      rdf:first [ rdf:type <http://www.w3.org/2003/11/swrl#IndividualPropertyAtom> ;
                                                                  <http://www.w3.org/2003/11/swrl#propertyPredicate> :wasAssociatedWith ;
                                                                  <http://www.w3.org/2003/11/swrl#argument1> <urn:swrl:var#y> ;
                                                                  <http://www.w3.org/2003/11/swrl#argument2> <urn:swrl:var#z>
                                                                ] ;
                                                      rdf:rest rdf:nil
                                                    ]
                                         ] ;
   <http://www.w3.org/2003/11/swrl#head> [ rdf:type <http://www.w3.org/2003/11/swrl#AtomList> ;
                                           rdf:first [ rdf:type <http://www.w3.org/2003/11/swrl#IndividualPropertyAtom> ;
                                                       <http://www.w3.org/2003/11/swrl#propertyPredicate> :wasAttributedTo ;
                                                       <http://www.w3.org/2003/11/swrl#argument1> <urn:swrl:var#x> ;
                                                       <http://www.w3.org/2003/11/swrl#argument2> <urn:swrl:var#z>
                                                     ] ;
                                           rdf:rest rdf:nil
                                         ]
 ] .
