@prefix : <https://w3id.org/pink#> .
@prefix owl: <http://www.w3.org/2002/07/owl#> .
@prefix rdf: <http://www.w3.org/1999/02/22-rdf-syntax-ns#> .
@prefix xml: <http://www.w3.org/XML/1998/namespace> .
@prefix xsd: <http://www.w3.org/2001/XMLSchema#> .
@prefix bibo: <http://purl.org/ontology/bibo/> .
@prefix foaf: <http://xmlns.com/foaf/0.1/> .
@prefix rdfs: <http://www.w3.org/2000/01/rdf-schema#> .
@prefix dcat: <http://www.w3.org/ns/dcat#> .
@prefix skos: <http://www.w3.org/2004/02/skos/core#> .
@prefix prov: <http://www.w3.org/ns/prov#> .
@prefix vann: <http://purl.org/vocab/vann/> .
@prefix dcatap: <http://data.europa.eu/r5r/> .
@prefix dcterms: <http://purl.org/dc/terms/> .
@prefix ddoc: <https://w3id.org/emmo/application/datadoc#> .

@base <https://w3id.org/pink#> .

<https://w3id.org/pink>
    rdf:type owl:Ontology ;
    owl:versionIRI <https://w3id.org/pink/0.0.1> ;
    owl:imports <https://w3id.org/pink/0.0.1/contributors> ,
                <https://w3id.org/pink/0.0.1/reused-terms> ;
    dcatap:status "Under Development" ;
    dcterms:abstract "The PINK Annotation Schema provides the semantic basis for SSbD."@en ;
    dcterms:bibliographicCitation "xxx" ;
    dcterms:contributor :IseultLynch ;
    dcterms:created "2025-09-08" ;
    dcterms:creator :FrancescaBleken ,
                    :JesperFriis ,
                    :JohDokler ,
                    :ThomasExner ;
    dcterms:hasFormat <https://www.w3.org/TR/turtle/> ;
    dcterms:issued "xxxx-xx-xx" ;
    dcterms:license "https://creativecommons.org/licenses/by/4.0/legalcode" ;
    dcterms:modified "xxxx-xx-xx" ;
    dcterms:publisher <https://pink-project.eu/> ;
    dcterms:source "Relevant PINK deliverable" ;
    dcterms:title "PINK Annotation Schema"@en ;
    bibo:doi "tbd" ;
    vann:preferredNamespacePrefix "pink" ;
    vann:preferredNamespaceUri "https://w3id.org/pink" ;
    rdfs:comment "This expands on the annotation schema provided by tripper, which again expands on the DCAT-AP."@en ;
    owl:priorVersion "0.0.0" ;
    owl:versionInfo "0.0.1" ;
    foaf:homepage <https://github.com/PINK-project/PINK-annotation-schema> ;
    foaf:logo <https://tess.elixir-europe.org/system/content_providers/images/000/000/777/original/pink-logo-orange-colorB-500.png> .

#################################################################
#    Annotation properties
#################################################################

###  http://data.europa.eu/r5r/status
dcatap:status rdf:type owl:AnnotationProperty .


###  http://purl.org/dc/terms/bibliographicCitation
dcterms:bibliographicCitation rdf:type owl:AnnotationProperty .


###  http://purl.org/dc/terms/contributor
dcterms:contributor rdf:type owl:AnnotationProperty .


###  http://purl.org/dc/terms/created
dcterms:created rdf:type owl:AnnotationProperty .


###  http://purl.org/dc/terms/creator
dcterms:creator rdf:type owl:AnnotationProperty .


###  http://purl.org/dc/terms/description
dcterms:description rdf:type owl:AnnotationProperty .


###  http://purl.org/dc/terms/hasFormat
dcterms:hasFormat rdf:type owl:AnnotationProperty .


###  http://purl.org/dc/terms/issued
dcterms:issued rdf:type owl:AnnotationProperty .


###  http://purl.org/dc/terms/modified
dcterms:modified rdf:type owl:AnnotationProperty .


###  http://purl.org/dc/terms/source
dcterms:source rdf:type owl:AnnotationProperty .


###  http://purl.org/ontology/bibo/doi
bibo:doi rdf:type owl:AnnotationProperty .


###  http://purl.org/vocab/vann/preferredNamespacePrefix
vann:preferredNamespacePrefix rdf:type owl:AnnotationProperty .


###  http://purl.org/vocab/vann/preferredNamespaceUri
vann:preferredNamespaceUri rdf:type owl:AnnotationProperty .


###  http://purl.org/vocab/vann/usageNote
vann:usageNote rdf:type owl:AnnotationProperty .


###  http://xmlns.com/foaf/0.1/homepage
foaf:homepage rdf:type owl:AnnotationProperty .


###  http://xmlns.com/foaf/0.1/logo
foaf:logo rdf:type owl:AnnotationProperty .


###  https://w3id.org/pink#conformance
:conformance rdf:type owl:ObjectProperty ;
    rdfs:range ddoc:ConformanceLevel ;
    dcterms:description "Whether the annotation is mandatory, recommended or optional as part of the PINK Annotation Schema"@en ;
    vann:usageNote "It MUST take one of the values 'ddoc:mandatory', 'ddoc:recommended' or 'ddoc:optional'."@en ;
    rdfs:isDefinedBy <https://w3id.org/pink> ;
    skos:prefLabel "conformance" .



#################################################################
#    Object properties
#################################################################

### SSbD relations

# TODO: Add rdfs:subPropertyOf
:ssbdCategory rdf:type owl:ObjectProperty ;
    rdfs:range :SsbdCategory ;
    skos:prefLabel "ssbdCategory"@en ;
    dcterms:description "XXX"@en ;
    vann:usageNote "One of `pink:functionality`, `pink:safety`, `pink:environmental_sustainability`, `pink:social_sustainability`"@en .

:ssbdSubCategory rdf:type owl:DatatypeProperty ;
    rdfs:range xsd:string ;
    skos:prefLabel "ssbdSubCategory"@en ;
    dcterms:description "XXX"@en .


### Other PINK-specific relations
:method a owl:ObjectProperty ;
    rdfs:domain :Dataset ;
    rdfs:range :Method ;
    skos:prefLabel "method"@en ;
    dcterms:description "Relates a dataset to the method that it was created with." .

:documentation a owl:ObjectProperty ;
    rdfs:domain dcat:Resource ;
    rdfs:range foaf:Document ;
    skos:prefLabel "documentation"@en ;
    dcterms:description "A page or document documenting this resource." .

:hasAPI a owl:DatatypeProperty ;
    rdfs:domain dcat:Resource ;
    rdfs:range xsd:boolean ;
    skos:prefLabel "hasAPI"@en ;
    dcterms:description "Whether the method has an API." .


### Parthood relations
:overlaps rdf:type owl:ObjectProperty, owl:SymmetricProperty, owl:ReflexiveProperty ;
    skos:prefLabel "overlaps"@en ;
    dcterms:description "The relation between two individuals representing entities that share at least one of their parts."@en .

:isOvercrossedBy rdf:type owl:ObjectProperty, owl:IrreflexiveProperty ;
    rdfs:subPropertyOf :overlaps ;
    skos:prefLabel "isOvercrossedBy"@en ;
    owl:propertyDisjointWith :hasPart ;
    dcterms:description "The relation between an entity that overlaps another without having it as part."@en .

:hasPart rdf:type owl:ObjectProperty, owl:ReflexiveProperty, owl:TransitiveProperty ;
    rdfs:subPropertyOf dcterms:hasPart, :overlaps ;
    skos:prefLabel "hasPart"@en ;
    dcterms:description "The primitive relation that express the concept of an entity being part of another one."@en .

:hasParticipant rdf:type owl:ObjectProperty, owl:IrreflexiveProperty, owl:AsymmetricProperty ;
    rdfs:subPropertyOf :hasPart ;
    skos:prefLabel "hasParticipant"@en ;
    dcterms:description "The relation between a process and an object participating to it, i.e. that is relevant to the process itself."@en ;
    rdfs:comment "Participation is a parthood relation: you must be part of the process to contribute to it. A participant whose 4D extension is totally contained within the process."@en .

:hasDatum rdf:type owl:ObjectProperty, owl:IrreflexiveProperty, owl:AsymmetricProperty ;
    rdfs:subPropertyOf :hasPart ;
    skos:prefLabel "hasDatum"@en ;
    dcterms:description "Relates a dataset to one of its datum."@en .

:hasSpatialPart rdf:type owl:ObjectProperty, owl:IrreflexiveProperty, owl:AsymmetricProperty ;
    rdfs:subPropertyOf :hasPart, :overcrosses ;
    skos:prefLabel "hasSpatialPart"@en ;
    dcterms:description "A proper part of a whole, whose parts always cover the full temporal extension of the whole within a spatial interval."@en ;
    rdfs:comment "The part is connected with the rest item or members with hasContact relations only (no hasNext)."@en .

:hasTemporalPart rdf:type owl:ObjectProperty, owl:IrreflexiveProperty, owl:AsymmetricProperty ;
    rdfs:subPropertyOf :hasPart, :overcrosses ;
    skos:prefLabel "hasTemporalPart"@en ;
    dcterms:description "A relation that identify a proper item part of the whole, whose parts always cover the full spatial extension of the whole within a time interval." ;
    rdfs:comment "A temporal part of an item cannot both cause and be caused by any other proper part of the item."@en .

:hasJunctionPart rdf:type owl:ObjectProperty, owl:IrreflexiveProperty, owl:AsymmetricProperty ;
    rdfs:subPropertyOf :hasPart, :overcrosses ;
    skos:prefLabel "hasJunctionPart"@en ;
    skos:altLabel "hasSpatioTemporalPart"@en ;
    dcterms:description "The part is connected with the rest item or members with both hasNext (or its inverse) and hasContact relations."@en .


:participatesTo rdf:type owl:ObjectProperty, owl:IrreflexiveProperty, owl:AsymmetricProperty ;
    rdfs:subPropertyOf :overcrosses ;
    skos:prefLabel "participatesTo"@en ;
    rdfs:domain prov:Entity ;
    rdfs:range prov:Activity ;
    rdfs:comment "The entity through overlaps the activity."@en ;
    dcterms:description "Relation an entity to an activity that it interacts with."@en .

:used rdf:type owl:ObjectProperty, owl:IrreflexiveProperty, owl:AsymmetricProperty ;
    rdfs:subPropertyOf prov:used, :overcrosses ;
    skos:prefLabel "used"@en ;
    rdfs:domain prov:Activity ;
    rdfs:range prov:Entity ;
    rdfs:comment "The activity A proper overlaps the entity E, where the non-overlapping part of E causes A."@en ;
    dcterms:description "Relates an activity to an entity that it used."@en ;
    skos:example "For example, :baking :used :spoon, :egg, :oven ." .

:wasGeneratedFrom rdf:type owl:ObjectProperty, owl:IrreflexiveProperty, owl:AsymmetricProperty ;
    rdfs:subPropertyOf prov:wasGeneratedFrom, :overcrosses ;
    skos:prefLabel "wasGeneratedFrom"@en ;
    rdfs:domain prov:Entity ;
    rdfs:range prov:Activity ;
    rdfs:comment "The activity A proper overlaps the entity E, where the non-overlapping part of E is caused by A."@en ;
    dcterms:description "Relates an entity to the activity it was generated from."@en .

:wasAssociatedWith rdf:type owl:ObjectProperty, owl:IrreflexiveProperty, owl:AsymmetricProperty ;
    rdfs:subPropertyOf prov:wasAssociatedWith, :overcrosses ;
    skos:prefLabel "wasAssociatedWith"@en ;
    rdfs:domain prov:Activity ;
    rdfs:range prov:Agent ;
    rdfs:comment "The activity is through overlapped by the agent."@en .
    dcterms:description "Relates an activity to an agent that had some (unspecified) responsibility for the occurence of this activity."@en .

:wasAttributedTo rdf:type owl:ObjectProperty, owl:IrreflexiveProperty, owl:AsymmetricProperty ;
    rdfs:subPropertyOf prov:wasAttributedTo, :overcrosses ;
    skos:prefLabel "wasAttributedTo"@en ;
    rdfs:domain prov:Entity ;
    rdfs:range prov:Agent ;
    rdfs:comment "The activity is through overlapped by the agent and overcrossed by the entity."@en ;
    dcterms:description "Relates an entity to an agent via an activity that both the entity and agent participates to."@en ;
    owl:inverseOf :attributed .

:attributed rdf:type owl:ObjectProperty, owl:IrreflexiveProperty, owl:AsymmetricProperty ;
    rdfs:subPropertyOf :overcrosses ;
    skos:prefLabel "attributed"@en ;
    rdfs:domain prov:Agent ;
    rdfs:range prov:Entity ;
    rdfs:comment "The activity is through overlapped by the agent and overcrossed by the entity."@en ;
    dcterms:description "Relates an agent to an entity via an activity that both the agent and entity participates to."@en ;
    owl:inverseOf :wasAttributedTo .

:process rdf:type owl:ObjectProperty, owl:IrreflexiveProperty, owl:AsymmetricProperty ;
    rdfs:subPropertyOf :participatesTo ;
    skos:prefLabel "process"@en ;
    rdfs:domain :Method ;
    rdfs:range :Process ;
    rdfs:comment "This is a subproperty of participatesTo, meaning that the process is overcrossed by the method."@en ;
    rdfs:comment "The starting point for this relation is that it relates a method to an activity it describes. However, when an activity is described by a method is a process. Therefor is the range of this relation a process and not only an activity."@en ;
    dcterms:description "Relates a method to the process that it describes."@en .

:input rdf:type owl:ObjectProperty, owl:IrreflexiveProperty, owl:AsymmetricProperty ;
    rdfs:subPropertyOf :attributed ;
    skos:prefLabel "input"@en ;
    rdfs:domain :Method ;
    rdfs:range prov:Entity ;
    rdfs:comment "The process P is through overlapped by the agent A and overcrossed by the entity E, where the non-overlapping part of E causes P."@en ;
    dcterms:description "Relates a method to an entity via a process that used the entity and that the method participates to."@en .

:output rdf:type owl:ObjectProperty, owl:IrreflexiveProperty, owl:AsymmetricProperty ;
    rdfs:subPropertyOf :attributed ;
    skos:prefLabel "output"@en ;
    rdfs:domain prov:Method ;
    rdfs:range prov:Entity ;
    rdfs:comment "The process P is through overlapped by the agent A and overcrossed by the entity E, where the non-overlapping part of E is caused by P."@en ;
    dcterms:description "Relates a method to an entity via a process that was generated by the entity and that the method participates to."@en .


### Causal relations
:causedBy rdf:type owl:ObjectProperty, owl:IrreflexiveProperty ;
    skos:prefLabel "causedBy"@en ;
    dcterms:description "A relation between an entity that causally affects the subject."@en ;
    skos:example "John yesterday is the cause of John today, is an example of temporal-like causality. The desk supporting my laptop is a space-like causality."@en .

:isAfter rdf:type owl:ObjectProperty, owl:IrreflexiveProperty, owl:AsymmetricProperty ;
    rdfs:subPropertyOf :causedBy ;
    skos:prefLabel "isAfter"@en ;
    dcterms:description "A one-directional relation between an entity that affects the subject."@en .

:processedFrom rdf:type owl:ObjectProperty, owl:IrreflexiveProperty, owl:AsymmetricProperty ;
    rdfs:subPropertyOf :isAfter ;
    skos:prefLabel "processedFrom"@en ;
    dcterms:description "Indirect relation that relates the output of an activity to its input."@en .

:wasInformedBy rdf:type owl:ObjectProperty, owl:IrreflexiveProperty, owl:AsymmetricProperty ;
    rdfs:subPropertyOf :isAfter, prov:wasInformedBy ;
    skos:prefLabel "wasInformedBy"@en ;
    dcterms:description "A one-directional relation between an activity that affects the subject activity."@en ;
    rdfs:domain prov:Activity ;
    rdfs:range prov:Activity .

:wasDerivedFrom rdf:type owl:ObjectProperty, owl:IrreflexiveProperty, owl:AsymmetricProperty ;
    rdfs:subPropertyOf :processedFrom, prov:wasDerivedFrom ;
    skos:prefLabel "wasDerivedFrom"@en ;
    dcterms:description "Indirect relation that relates the output entity of an activity to its input entity."@en ;
    rdfs:domain prov:Entity ;
    rdfs:range prov:Entity .


### Other relations
:hasProperty rdf:type owl:ObjectProperty ;
    skos:prefLabel "hasProperty"@en ;
    dcterms:description "A semiotic relation that connects a semiotic object to a property in a declaration process."@en ;
    rdfs:domain prov:Entity ;
    rdfs:range :Property .


#################################################################
#    Classes
#################################################################

### SSbD-related classes
:SsbdCategory rdf:type owl:Class ;
    skos:prefLabel "SsbdCategory"@en ;
    rdfs:comment "The pink:SsbdCategory is an extension of the 'sustainability dimensions' defined by JRC." ;
    dcterms:description "XXX"@en .

:Method rdf:type owl:Class ;
    rdfs:subClassOf :Data ;
    skos:prefLabel "Method"@en ;
    dcterms:description "Data that describes how to perform an activity."@en .

:Process rdf:type owl:Class ;
    rdfs:subClassOf prov:Activity, [
        rdf:type owl:Restriction ;
        owl:onProperty [ owl:inverseOf :isMethodFor ] ;
        owl:someValuesFrom :Method
    ] ;
    skos:prefLabel "Process"@en ;
    dcterms:description "An activity that is described by a method."@en .


### General classes
:Role rdf:type owl:Class ;
    skos:prefLabel "Role"@en ;
    dcterms:description "The class of all individuals that are defined through a parthood relation to an entity."@en ;
    vann:usageNote "An individual can be said to have a role in relation to the entity."@en .

:MaterialProcess rdf:type owl:Class ;
    rdfs:subClassOf :Process ;
    skos:prefLabel "MaterialProcess"@en ;
    rdfs:comment "Since MaterialProcess is a subclass of Process, we say that there must exist a method that describes the material process." ;
    dcterms:description "A process that has material as input and output."@en .

:Measurement rdf:type owl:Class ;
    rdfs:subClassOf :Process ;
    skos:prefLabel "Measurement"@en ;
    rdfs:comment "Since Measurement is a subclass of Process, we say that there must exist a method that describes the measurement." ;
    dcterms:description "An observation that results in a quantitative comparison of a 'property' of an 'object' with a standard reference based on a well defined mesurement procedure."@en .

:Computation rdf:type owl:Class ;
    rdfs:subClassOf :Process ;
    skos:prefLabel "Computation"@en ;
    rdfs:comment "Since Computation is a subclass of Process, we say that there must exist a method that describes the computation." ;
    dcterms:description "A procedure that deals with quantitative symbols (i.e. symbols associated with a quantitative oriented language)."@en .

:Material rdf:type owl:Class ;
    rdfs:subClassOf prov:Entity ;
    skos:prefLabel "Material"@en ;
    dcterms:description "The class of individuals standing for an amount of matter (ordinary, anti or hybrid) substance (or mixture of substances) in different states of matter or phases."@en .

:Property rdf:type owl:Class ;
    rdfs:subClassOf prov:Entity ;
    skos:prefLabel "Property"@en ;
    dcterms:description "A coventional semiotic sigh that stands for an physical interaction with an object using an atomic symbol."@en ;
    vann:usageNote "A property is atomic in the sense that is aimed to deliver one and one only aspect of the object."@en .

:Data rdf:type owl:Class ;
    rdfs:subClassOf prov:Entity ;
    skos:prefLabel "Data"@en ;
    dcterms:description "Contrast from variation of properties that is encoded by an agent and that can be decoded by another agent according to a specific rule."@en .

:Object rdf:type owl:Class ;
    rdfs:subClassOf prov:Entity ;
    skos:prefLabel "Object"@en ;
    dcterms:description "The class of all individuals who's temporal parts are of the same type as the whole."@en .

:Datum rdf:type owl:Class ;
    rdfs:subClassOf :Data ;
    skos:prefLabel "Datum"@en ;
    dcterms:description "A self-consistent encoded data entity."@en ;
    vann:usageNote "Datum is the building block of datasets."@en .

:ReliabilityDocument rdf:type owl:Class ;
    rdfs:subClassOf foaf:Document ;
    skos:prefLabel "ReliabilityDocument"@en ;
    dcterms:description "xxx"@en ;
    vann:usageNote "xxx"@en .

:Participant rdf:type owl:Class ;
    rdfs:subClassOf :Object, prov:Agent ;
    skos:prefLabel "Participant"@en ;
    dcterms:description "An object which is a spatial part of a process."@en ;
    vann:usageNote "Example: A student during an examination. The student exists both before and after the examination."@en .

:Dataset rdf:type owl:Class ;
    rdfs:subClassOf dcat:Dataset, :Data, [
        rdf:type owl:Restriction ;
        owl:onProperty :hasPart ;
        owl:someValuesFrom :Datum
    ] ;
    skos:prefLabel "Dataset"@en ;
    dcterms:description "Encoded data made of more than one datum."@en ;
    vann:usageNote "A collection of (more than one) datum, published or curated by a single agent, and available for access or download in one or more representations."@en .


### Include standard concepts into the PINK taxonomy
### Question: should we duplicate these classes instead?
foaf:Document rdfs:subClassOf :Data .
prov:Agent rdfs:subClassOf :Role .


#################################################################
#    Individuals
#################################################################

### Conformance individuals
ddoc:mandatory rdf:type owl:NamedIndividual ;
    skos:prefLabel "mandatory"@en .

ddoc:optional rdf:type owl:NamedIndividual ;
    skos:prefLabel "optional"@en .

ddoc:recommended rdf:type owl:NamedIndividual ;
    skos:prefLabel "recommended"@en .


### SSbD categories
:functionality a :SsbdCategory ;
    skos:prefLabel: "functionality" ;
    dcterms:description "XXX"@en .

:safety a :SsbdCategory ;
    skos:prefLabel: "safety" ;
    dcterms:description "Human helth and environmental safety aspects of chemicals and materials."@en ;
    dcterms:bibliographicCitation "Caldeira et al. JRC Technical Report. Sage and Sustainable by Design chemicals and materials. EU Science Hub. doi:10.2760/487955. 2022" ;
    rdfs:comment """In the context of chemicals assessment, safety could be referring to a
certain condition where a stressor (e.g. a chemical) is unlikely to
cause any adverse effect to a receptor (e.g. humans and other
organisms) (more related to intrinsic hazard properties of the
stressor) or where a receptor is protected from risk (more related to
control measures or mechanisms to minimise exposure to the
stressor). In any case, the term safe involves receptors, and with
that generally also requires the consideration of the contact
(i.e. exposure) between stressors and receptors as addressed in a risk
assessment context."""@en .

:environmental_systainability a :SsbdCategory ;
    skos:prefLabel: "environmental_systainability" ;
    dcterms:description "The ability to conserve natural resources and protect global ecosystems to support human health and wellbeing, within the limits of our Planet"@en ;
    dcterms:bibliographicCitation "Caldeira et al. JRC Technical Report. Sage and Sustainable by Design chemicals and materials. EU Science Hub. doi:10.2760/487955. 2022" ;
    rdfs:comment """Assessing environmental sustainability implies to assess the environmental impacts generated by
chemicals/materials along the entire life cycle to move towards:

  路 A toxic-free environment as stated in the CSS (i.e. minimising the total toxicity footprint in terms
    of ecotoxicity and human toxicity13 - at each stage of the production and consumption life cycle,
    originated not only by the assessed chemical or material, but also by all the chemicals that are emitted
    along the life cycle14) (EC, 2020a);
  路 A climate-neutral economy (i.e. minimising the emission of greenhouse gases along the life cycle)
    (EC, 2019b);
  路 A resource efficient economy and a regenerative economy (i.e. using natural resources in a
    sustainable manner, minimising inputs and waste generation, and providing more benefits than
    burdens) (EC, 2020b);
  路 The reduction of biodiversity loss and the conservation of ecosystem functioning, addressing the
    main drivers of structural and functional biodiversity loss (e.g. land use, climate change) (EC, 2020c);
"""@en .

:social_systainability a :SsbdCategory ;
    skos:prefLabel: "social_sustainability" ;
    dcterms:description "A globally agreed list of objectives and targets to be pursued for achieving sustainable development."@en ;
    dcterms:bibliographicCitation "Caldeira et al. JRC Technical Report. Sage and Sustainable by Design chemicals and materials. EU Science Hub. doi:10.2760/487955. 2022" ;
    rdfs:comment """In the SDGs framework several Goals focus on social aspects,
e.g. poverty eradication (SDG 1), food security (SDG 2), health (SDG 3),
education (SDG 4), gender equality (SDG 5), decent work (SDG 8),
reduce inequalities (SDG 10), peace and justice (SDG 16)."""@en .

:economic a :SsbdCategory ;
    skos:prefLabel: "economic" ;
    dcterms:description "Aspects related to techno-economic feasibility, to operational costs, etc."@en ;
    dcterms:bibliographicCitation "Caldeira et al. JRC Technical Report. Sage and Sustainable by Design chemicals and materials. EU Science Hub. doi:10.2760/487955. 2022" ;
    rdfs:comment """There are important considerations to be made in the context of SSbD
such as the 'availability' of raw materials, as chemicals/materials
cannot be declared SSbD if the raw materials to produce them are not
renewable or are (very) scarce and extracted and processed in an
unsustainable manner. Economic aspects play a role when there is a
need to rank chemicals and materials based on SSbD criteria (even if
they are not SSbD). However, mainly externalities consideration is at
stake in a sustainability framework like the SSbD one."""@en .


#################################################################
#    Rules
#################################################################

<urn:swrl:var#x> rdf:type <http://www.w3.org/2003/11/swrl#Variable> .

<urn:swrl:var#y> rdf:type <http://www.w3.org/2003/11/swrl#Variable> .

<urn:swrl:var#z> rdf:type <http://www.w3.org/2003/11/swrl#Variable> .

[ rdf:type <http://www.w3.org/2003/11/swrl#Imp> ;
   <http://www.w3.org/2003/11/swrl#body> [ rdf:type <http://www.w3.org/2003/11/swrl#AtomList> ;
                                           rdf:first [ rdf:type <http://www.w3.org/2003/11/swrl#IndividualPropertyAtom> ;
                                                       <http://www.w3.org/2003/11/swrl#propertyPredicate> :wasGeneratedBy ;
                                                       <http://www.w3.org/2003/11/swrl#argument1> <urn:swrl:var#x> ;
                                                       <http://www.w3.org/2003/11/swrl#argument2> <urn:swrl:var#y>
                                                     ] ;
                                           rdf:rest [ rdf:type <http://www.w3.org/2003/11/swrl#AtomList> ;
                                                      rdf:first [ rdf:type <http://www.w3.org/2003/11/swrl#IndividualPropertyAtom> ;
                                                                  <http://www.w3.org/2003/11/swrl#propertyPredicate> :used ;
                                                                  <http://www.w3.org/2003/11/swrl#argument1> <urn:swrl:var#y> ;
                                                                  <http://www.w3.org/2003/11/swrl#argument2> <urn:swrl:var#z>
                                                                ] ;
                                                      rdf:rest rdf:nil
                                                    ]
                                         ] ;
   <http://www.w3.org/2003/11/swrl#head> [ rdf:type <http://www.w3.org/2003/11/swrl#AtomList> ;
                                           rdf:first [ rdf:type <http://www.w3.org/2003/11/swrl#IndividualPropertyAtom> ;
                                                       <http://www.w3.org/2003/11/swrl#propertyPredicate> :processedFrom ;
                                                       <http://www.w3.org/2003/11/swrl#argument1> <urn:swrl:var#x> ;
                                                       <http://www.w3.org/2003/11/swrl#argument2> <urn:swrl:var#z>
                                                     ] ;
                                           rdf:rest rdf:nil
                                         ]
 ] .

[ rdf:type <http://www.w3.org/2003/11/swrl#Imp> ;
   <http://www.w3.org/2003/11/swrl#body> [ rdf:type <http://www.w3.org/2003/11/swrl#AtomList> ;
                                           rdf:first [ rdf:type <http://www.w3.org/2003/11/swrl#IndividualPropertyAtom> ;
                                                       <http://www.w3.org/2003/11/swrl#propertyPredicate> :wasGeneratedBy ;
                                                       <http://www.w3.org/2003/11/swrl#argument1> <urn:swrl:var#x> ;
                                                       <http://www.w3.org/2003/11/swrl#argument2> <urn:swrl:var#y>
                                                     ] ;
                                           rdf:rest [ rdf:type <http://www.w3.org/2003/11/swrl#AtomList> ;
                                                      rdf:first [ rdf:type <http://www.w3.org/2003/11/swrl#IndividualPropertyAtom> ;
                                                                  <http://www.w3.org/2003/11/swrl#propertyPredicate> :used ;
                                                                  <http://www.w3.org/2003/11/swrl#argument1> <urn:swrl:var#y> ;
                                                                  <http://www.w3.org/2003/11/swrl#argument2> <urn:swrl:var#z>
                                                                ] ;
                                                      rdf:rest rdf:nil
                                                    ]
                                         ] ;
   <http://www.w3.org/2003/11/swrl#head> [ rdf:type <http://www.w3.org/2003/11/swrl#AtomList> ;
                                           rdf:first [ rdf:type <http://www.w3.org/2003/11/swrl#IndividualPropertyAtom> ;
                                                       <http://www.w3.org/2003/11/swrl#propertyPredicate> :wasDerivedFrom ;
                                                       <http://www.w3.org/2003/11/swrl#argument1> <urn:swrl:var#x> ;
                                                       <http://www.w3.org/2003/11/swrl#argument2> <urn:swrl:var#z>
                                                     ] ;
                                           rdf:rest rdf:nil
                                         ]
 ] .

[ rdf:type <http://www.w3.org/2003/11/swrl#Imp> ;
   <http://www.w3.org/2003/11/swrl#body> [ rdf:type <http://www.w3.org/2003/11/swrl#AtomList> ;
                                           rdf:first [ rdf:type <http://www.w3.org/2003/11/swrl#IndividualPropertyAtom> ;
                                                       <http://www.w3.org/2003/11/swrl#propertyPredicate> :used ;
                                                       <http://www.w3.org/2003/11/swrl#argument1> <urn:swrl:var#x> ;
                                                       <http://www.w3.org/2003/11/swrl#argument2> <urn:swrl:var#y>
                                                     ] ;
                                           rdf:rest [ rdf:type <http://www.w3.org/2003/11/swrl#AtomList> ;
                                                      rdf:first [ rdf:type <http://www.w3.org/2003/11/swrl#IndividualPropertyAtom> ;
                                                                  <http://www.w3.org/2003/11/swrl#propertyPredicate> :wasGeneratedBy ;
                                                                  <http://www.w3.org/2003/11/swrl#argument1> <urn:swrl:var#y> ;
                                                                  <http://www.w3.org/2003/11/swrl#argument2> <urn:swrl:var#z>
                                                                ] ;
                                                      rdf:rest rdf:nil
                                                    ]
                                         ] ;
   <http://www.w3.org/2003/11/swrl#head> [ rdf:type <http://www.w3.org/2003/11/swrl#AtomList> ;
                                           rdf:first [ rdf:type <http://www.w3.org/2003/11/swrl#IndividualPropertyAtom> ;
                                                       <http://www.w3.org/2003/11/swrl#propertyPredicate> :wasInformedBy ;
                                                       <http://www.w3.org/2003/11/swrl#argument1> <urn:swrl:var#x> ;
                                                       <http://www.w3.org/2003/11/swrl#argument2> <urn:swrl:var#z>
                                                     ] ;
                                           rdf:rest rdf:nil
                                         ]
 ] .


###  Generated by the OWL API (version 4.5.29.2024-05-13T12:11:03Z) https://github.com/owlcs/owlapi
